theories/iris/logrel/load_common.v
@@ -1,0 +1,1848 @@
+From mathcomp Require Import eqtype ssrbool.
+
+From Stdlib Require Import NArith.NArith.
+Require Import RichWasm.util.
+Require Import RichWasm.compiler.memory.
+Require Import RichWasm.iris.numerics.
+Require Import RichWasm.iris.runtime.
+Require Import RichWasm.iris.logrel.instr.typing.common.
+Require Import RichWasm.iris.logrel.case_ptr.
+Require Import RichWasm.iris.logrel.path.
+Require Import RichWasm.iris.logrel.roots.
+Require Import RichWasm.iris.logrel.rt_token.
+
+Set Bullet Behavior "Strict Subproofs".
+Set Default Goal Selector "!".
+
+Section load_common.
+
+  Context `{!logrel_na_invs Σ}.
+  Context `{!wasmG Σ}.
+  Context `{!richwasmG Σ}.
+
+  Variable rti : rt_invariant Σ.
+  Variable sr : store_runtime.
+  Variable mr : module_runtime.
+
+
+  Lemma atoms_interp_nil_inv vs :
+    atoms_interp [] vs ⊣⊢ ⌜vs = []⌝ .
+  Proof.
+    iSplit.
+    - setoid_rewrite big_sepL2_nil_inv_l.
+      done.
+    - iIntros (->); cbn; done.
+  Qed.
+
+  Lemma atoms_interp_cons_inv o os vs :
+    ⊢ atoms_interp (o :: os) vs -∗ ∃ v vs', ⌜vs = v :: vs'⌝ ∗ atom_interp o v ∗ atoms_interp os vs'.
+  Proof.
+    iIntros "Hat".
+    iEval (unfold atoms_interp) in "Hat".
+    setoid_rewrite big_sepL2_cons_inv_l.
+    iDestruct "Hat" as (v vs' Hvs) "(Hv & Hvs')".
+    iExists v, vs'; iFrame; done.
+  Qed.
+
+  Lemma atoms_interp_length os vs :
+    ⊢ atoms_interp os vs -∗ ⌜length os = length vs⌝.
+  Proof.
+    iApply big_sepL2_length.
+  Qed.
+
+  Lemma atoms_interp_one_inv o vs :
+    atoms_interp [o] vs ⊣⊢ ∃ v, ⌜vs = [v]⌝ ∗ atom_interp o v.
+  Proof.
+    iSplit.
+    - iIntros "Hvs".
+      iPoseProof (atoms_interp_cons_inv with "Hvs") as (v vs' Heq) "[Hv Hnil]".
+      rewrite atoms_interp_nil_inv.
+      iDestruct "Hnil" as "%Hnil"; subst.
+      iExists v; auto.
+    - iIntros "(%v & -> & Hv)".
+      cbn; auto.
+  Qed.
+
+  Lemma rep_ref_kind_ptr F κ μ β τ ρ ξ :
+    has_kind F (RefT κ μ β τ) (VALTYPE ρ ξ) ->
+    ρ = AtomR PtrR /\ exists ξ', κ = VALTYPE (AtomR PtrR) ξ'.
+  Proof.
+    intros Hkind.
+    remember (RefT κ μ β τ) as ref.
+    remember (VALTYPE ρ ξ) as val.
+    revert Heqval Heqref.
+    revert ρ ξ.
+    induction Hkind using has_kind_ind'; intros; try congruence.
+    - subst κ0.
+      split; try congruence.
+      inversion Heqref; eauto.
+    - subst κ0.
+      split; try congruence.
+      inversion Heqref; eauto.
+    - subst κ0.
+      split; try congruence.
+      inversion Heqref; eauto.
+  Qed.
+
+  Lemma Z_even_mod_even :
+    forall n k : Z,
+    Z.even k = true ->
+    Z.even (n mod k) = Z.even n.
+  Proof.
+    intros n k Hk.
+    apply Bool.eq_true_iff_eq.
+
+    assert (Hk2 : (k mod 2)%Z = 0).
+    { rewrite Zmod_even. by rewrite Hk. }
+    destruct (Z.eq_dec k 0) as [Hk0 | Hk0].
+    { subst. by rewrite Zmod_0_r. }
+
+    rewrite (Z.mod_eq n k); last done.
+
+    replace (n - k * (n / k))%Z with (n + (k * -(n / k)))%Z; last lia.
+    rewrite Z.even_add_mul_even.
+    2: { rewrite <- Z.even_spec. rewrite Zeven_mod. lia. }
+    done.
+  Qed.
+
+  Lemma Z_Even_mod_Even :
+    forall n k, Z.Even k -> Z.Even (n mod k) <-> Z.Even n.
+  Proof.
+    intros n k Hk.
+    do 2 rewrite <- Z.even_spec.
+    rewrite Z_even_mod_even; first done.
+    by apply Z.even_spec.
+  Qed.
+
+  Lemma Z_mod_even_mod_2 :
+    forall n k,
+    Z.Even k ->
+    ((n mod k) mod 2)%Z = (n mod 2)%Z.
+  Proof.
+    intros n k Hk.
+    rewrite Zmod_even.
+    rewrite Z_even_mod_even; last by rewrite Z.even_spec.
+    symmetry.
+    apply Zmod_even.
+  Qed.
+
+  Lemma mod32_mod2 (n: Z) :
+    (((2 * n) mod 4294967296) mod 2)%Z = 0.
+  Proof.
+    rewrite Z_mod_even_mod_2; last by rewrite <- Z.even_spec.
+    rewrite Zmod_even.
+    by rewrite Z.even_even.
+  Qed.
+
+  Lemma wp_load_w_strict μ t off wt wl wt' wl' es ret :
+    run_codegen (load_w mr μ t off) wt wl = inr (ret, wt', wl', es) ->
+    ret = () /\
+    wt' = [] /\
+    wl' = [] /\
+    forall ℓ ℓ32 memidx memidxN (f: frame) B R Φ v,
+        N_i32_repr ℓ ℓ32 ->
+        N_nat_repr memidx memidxN ->
+        inst_memory (f_inst f) !! base_mem_idx mr μ = Some memidx ->
+        types_agree t v ->
+        ⊢ ∀ s E,
+          ↪[frame] f -∗
+          ↪[RUN] -∗
+          memidxN ↦[wms][ℓ + byte_offset μ off]bits v -∗
+          ▷ (memidxN↦[wms][ℓ + byte_offset μ off]bits v -∗ Φ f [v]) -∗
+          CWP W.BI_const (VAL_int32 ℓ32) :: es @ s; E UNDER B; R {{ Φ }}.
+  Proof.
+    intros Hcg.
+    unfold load_w in Hcg.
+    inv_cg_emit Hcg; subst es wt' wl' ret.
+    split; [auto|].
+    split; [auto|].
+    split; [auto|].
+    intros * Hℓ Hmemidx Hmem Hty.
+    iIntros (s E) "Hf Hrun Hptr HΦ".
+    iApply (cwp_load with "[$] [$] [$] [$]"); eauto.
+  Qed.
+
+  Lemma mod_bound_nonzero (a b : N) :
+    (a <> 0 ->
+     a `mod` b = 0 ->
+     b <= a)%N.
+  Proof using.
+  Admitted.
+
+  (* This version is looser about the offset in the points-to,
+     but it needs to know that l mod 4 = 0 and l <> 0. *)
+  Lemma wp_load_w μ t off wt wl wt' wl' es ret :
+    run_codegen (load_w mr μ t off) wt wl = inr (ret, wt', wl', es) ->
+    ret = () /\
+    wt' = [] /\
+    wl' = [] /\
+    forall ℓ ℓ32 memidx memidxN (f: frame) B R Φ v,
+        N_i32_repr (tag_address μ ℓ)%N ℓ32 ->
+        N_nat_repr memidx memidxN ->
+        inst_memory (f_inst f) !! base_mem_idx mr μ = Some memidx ->
+        (ℓ `mod` 4 = 0)%N ->
+        (ℓ <> 0)%N ->
+        types_agree t v ->
+        ⊢ ∀ s E,
+          ↪[frame] f -∗
+          ↪[RUN] -∗
+          memidxN ↦[wms][ℓ + 4 * N.of_nat off] bits v -∗
+          ▷ (memidxN↦[wms][ℓ + 4 * N.of_nat off] bits v -∗ Φ f [v]) -∗
+          CWP W.BI_const (VAL_int32 ℓ32) :: es @ s; E UNDER B; R {{ Φ }}.
+  Proof.
+    intros Hcg.
+    apply wp_load_w_strict in Hcg.
+    intuition.
+    iIntros (s E) "Hf Hrun Hv Hpost".
+    assert (4 <= ℓ)%N.
+    {
+      by eapply mod_bound_nonzero.
+    }
+    assert ((ℓ + 4 * N.of_nat off = tag_address μ ℓ + byte_offset μ off)%N) as Heq.
+    {
+      destruct μ; cbn; unfold offset_mm, offset_gc; lia.
+    }
+    rewrite Heq.
+    iApply (H3 with "[$] [$] [Hv] [Hpost]"); eauto.
+  Qed.
+
+
+  Lemma wp_ite_gc_ptr_ptr_cg_state i ts1 ts2 do_gc do_nongc ret wt wl wt' wl' es:
+    run_codegen (ite_gc_ptr PtrR i (W.Tf ts1 ts2) do_gc do_nongc) wt wl = inr (ret, wt', wl', es) ->
+    ∃ wt1 wt2 wt3 wl1 wl2 wl3 es1 es2 es3,
+      run_codegen do_nongc wt wl = inr ((), wt1, wl1, es1) ∧
+      run_codegen do_nongc (wt ++ wt1) (wl ++ wl1) = inr ((), wt2, wl2, es2) /\
+        run_codegen do_gc (wt ++ wt1 ++ wt2) (wl ++ wl1 ++ wl2) = inr ((), wt3, wl3, es3) /\
+      wt' = wt1 ++ wt2 ++ wt3 /\
+      wl' = wl1 ++ wl2 ++ wl3.
+  Proof.
+    unfold ite_gc_ptr.
+    intros Hcg.
+    apply wp_ignore in Hcg.
+    destruct Hcg as ([] & [ [] [[] []]] & Hcg).
+    eapply cwp_case_ptr in Hcg; eauto.
+    destruct Hcg as (?wt & ?wt & ?wt & ?wl & ?wl & ?wl & ?es & ?es & ?es & Hcg).
+    destruct ret.
+    exists wt0, wt1, wt2, wl0, wl1, wl2, es0, es1, es2.
+    destruct Hcg as (Hnon1 & Hnon2 & Hgc & Hwt' & Hwl' & Hspec).
+    eauto.
+  Qed.
+
+
+  Lemma wp_ite_gc_ptr_ptr i ts1 ts2 do_gc do_nongc ret wt wl wt' wl' es evs vs s E R L Φ f ptr n n32:
+    run_codegen (ite_gc_ptr PtrR i (W.Tf ts1 ts2) do_gc do_nongc) wt wl = inr (ret, wt', wl', es) ->
+    has_values evs vs ->
+    length ts1 = length vs ->
+    ptr_shaped ptr n ->
+    N_i32_repr n n32 ->
+    ∃ wt1 wt2 wt3 wl1 wl2 wl3 es1 es2 es3,
+      run_codegen do_nongc wt wl = inr ((), wt1, wl1, es1) ∧
+      run_codegen do_nongc (wt ++ wt1) (wl ++ wl1) = inr ((), wt2, wl2, es2) /\
+      run_codegen do_gc (wt ++ wt1 ++ wt2) (wl ++ wl1 ++ wl2) = inr ((), wt3, wl3, es3) /\
+      wt' = wt1 ++ wt2 ++ wt3 /\
+      wl' = wl1 ++ wl2 ++ wl3 ∧
+      ⊢ ↪[frame]f -∗
+         ↪[RUN] -∗
+        ⌜f_locs f !! localimm i = Some (VAL_int32 n32)⌝ -∗
+        ▷ ( ↪[frame]f -∗
+            ↪[RUN] -∗
+           match ptr with
+           | PtrInt _ => CWP evs ++ es1 @ s; E UNDER []; R {{ f; vs, Φ f vs }}
+           | PtrHeap MemMM _ => CWP evs ++ es2 @ s; E UNDER []; R {{ f; vs, Φ f vs }}
+           | PtrHeap MemGC _ => CWP evs ++ es3 @ s; E UNDER []; R {{ f; vs, Φ f vs }}
+           end) -∗
+        CWP evs ++ es @ s; E UNDER L; R {{ f; vs, Φ f vs }}.
+  Proof.
+    unfold ite_gc_ptr.
+    intros Hcg Hevs Hlen.
+    apply wp_ignore in Hcg.
+    destruct Hcg as ([] & [ [] [[] []]] & Hcg).
+    eapply cwp_case_ptr in Hcg; eauto.
+    destruct Hcg as (?wt & ?wt & ?wt & ?wl & ?wl & ?wl & ?es & ?es & ?es & Hcg).
+    destruct ret.
+    exists wt0, wt1, wt2, wl0, wl1, wl2, es0, es1, es2.
+    destruct Hcg as (Hnon1 & Hnon2 & Hgc & Hwt' & Hwl' & Hspec).
+    split; first auto.
+    split; first auto.
+    split; first auto.
+    split; first auto.
+    split; first auto.
+    iIntros "Hf Hrun %Hi Hbr".
+    by iApply (Hspec with "[$] [$] [//] [$]").
+  Qed.
+
+  Lemma wp_ite_gc_ptr_nonptr ι i ts1 ts2 do_gc do_nongc ret wt wl wt' wl' es :
+    ι <> PtrR ->
+    run_codegen (ite_gc_ptr ι i (W.Tf ts1 ts2) do_gc do_nongc) wt wl = inr (ret, wt', wl', es) ->
+    run_codegen (do_nongc) wt wl = inr (ret, wt', wl', es).
+  Proof.
+    intros Hι Hcg.
+    destruct ι; solve [exfalso; by apply Hι | by apply Hcg].
+  Qed.
+
+  Lemma arep_types_agree ι o v :
+    has_arep ι o ->
+    atom_interp o v -∗
+    ⌜types_agree (translate_arep ι) v⌝.
+  Proof.
+    destruct ι, o; cbn;
+      iIntros "%Harep ->" || iIntros "%Harep Hat";
+      auto.
+    iDestruct "Hat" as "(%n & %n32 & %nrep & -> & _)".
+    auto.
+  Qed.
+
+  Definition mk_load1_frame fe f vloc v :=
+    let vloc := localimm (W.Mk_localidx (fe_wlocal_offset fe + vloc)) in
+    {| f_locs := <[vloc := v]> (f_locs f);
+       f_inst := f_inst f |}.
+
+  Lemma mk_load1_frame_stable_part fe f vloc v :
+    ∀ i,
+      i < fe_wlocal_offset fe + vloc ->
+      f_locs (mk_load1_frame fe f vloc v) !! i = f_locs f !! i.
+  Proof.
+    intros i Hlt.
+    cbn.
+    rewrite list_lookup_insert_ne; [done | lia].
+  Qed.
+
+  Definition mk_load1_post lmask o v v' : iProp Σ :=
+    (∃ e', rt_token rti sr lmask e' ∗
+           atom_interp o v ∗
+           atom_interp o v')%I.
+
+  Definition congeal32 (ns : list i32) : option i32 :=
+    match ns with
+    | [n] => Some n
+    | _ => None
+    end.
+
+  Definition congeal64 (ns : list i32) : option i64 :=
+    match ns with
+    | [n1; n2] =>
+        let n1' := Wasm_int.Int32.unsigned n1 in
+        let n2' := Wasm_int.Int32.unsigned n2 in
+        Some (Wasm_int.Int64.repr (Z.shiftl n1' 32 + n2'))
+    | _ => None
+    end.
+
+  Definition mk_float32 (i : i32) : f32 :=
+    Wasm_float.FloatSize32.of_bits
+      {| Integers.Int.intval := Wasm_int.Int32.intval i;
+         Integers.Int.intrange := unkeyed (Wasm_int.Int32.intrange i) |}.
+
+  Definition mk_float64 (i : i64) : f64 :=
+    Wasm_float.FloatSize64.of_bits
+      {| Integers.Int64.intval := Wasm_int.Int64.intval i;
+         Integers.Int64.intrange := unkeyed (Wasm_int.Int64.intrange i) |}.
+
+  Definition congeal_atom (ι : atomic_rep) (ns32 : list i32) : option value :=
+    match ι with
+    | PtrR
+    | I32R => option_map VAL_int32 (congeal32 ns32)
+    | I64R => option_map VAL_int64 (congeal64 ns32)
+    | F32R => option_map (VAL_float32 ∘ mk_float32) (congeal32 ns32)
+    | F64R => option_map (VAL_float64 ∘ mk_float64) (congeal64 ns32)
+    end.
+
+  Definition congeal_atoms (ιs : list atomic_rep) (nss32 : list (list i32)) : option (list value) :=
+    mapM (curry congeal_atom) (zip ιs nss32).
+
+  Lemma congeal_types_agree ι ns32 v :
+    congeal_atom ι ns32 = Some v ->
+    types_agree (translate_arep ι) v.
+  Proof.
+    induction ι; cbn; intros Hcong; destruct ns32 as [| ? [| ? [| ? ]]]; try done;
+      cbn in Hcong; inversion Hcong; subst; done.
+  Qed.
+
+  Lemma gc_word_to_atom ι o ns ns32 v θ :
+    ref_flag_atoms_interp GCRefs (SAtoms [o]) ->
+    Forall2 N_i32_repr ns ns32 ->
+    has_arep ι o ->
+    congeal_atom ι ns32 = Some v ->
+    words_interp θ MemMM (serialize_atom o) ns -∗
+    atom_interp o v.
+  Proof.
+    intros Href Hns Harep Hv.
+    iIntros "Hw".
+    destruct o, ι; cbn in Harep; try done.
+    - inversion Href; subst.
+      cbn in *.
+      destruct ns32 as [| n32 [| n' ns']];
+        cbn in Hv; inversion Hv; subst.
+      apply Forall2_cons_inv_r in Hns.
+      destruct Hns as (n & ns' & Hnrep & Hbad & ->).
+      inversion Hbad; subst.
+      rewrite big_sepL2_singleton.
+      cbn.
+      destruct p as [ | [|]]; cbn in *; try done.
+      + iDestruct "Hw" as "%Hw".
+        inversion Hw; subst.
+        rename n0 into n.
+        iExists (2 * n)%N, n32.
+        iSplit; eauto.
+        iSplit; eauto.
+        iExists (RootInt n).
+        cbn.
+        iPureIntro; split; eauto.
+        constructor.
+      + iDestruct "Hw" as "(%a & %Ha & Hroot)".
+        iExists _, _; eauto.
+    - cbn.
+      iPoseProof (big_sepL2_cons_inv_l with "Hw") as "(%n' & %ns' & %Hns' & Hn & Hns)".
+      cbn.
+      iPoseProof (big_sepL2_nil_inv_l with "Hns") as "->".
+      subst.
+      iDestruct "Hn" as "->".
+      destruct ns32 as [| ? [| ? ?]]; cbn in Hv; inversion Hv; subst.
+      inversion Hns; subst.
+      iPureIntro. f_equal.
+      eapply N_i32_repr_inj2; eauto.
+      done.
+    - admit.
+    - cbn.
+      iPoseProof (big_sepL2_cons_inv_l with "Hw") as "(%n' & %ns' & %Hns' & Hn & Hns)".
+      cbn.
+      iPoseProof (big_sepL2_nil_inv_l with "Hns") as "->".
+      subst.
+      iDestruct "Hn" as "->".
+      destruct ns32 as [| ? [| ? ?]]; cbn in Hv; inversion Hv; subst.
+      inversion Hns; subst.
+      iPureIntro.
+      admit.
+    - admit.
+  Admitted.
+
+  Definition mk_load1_frame' fe f vloc v :=
+    let vloc := localimm (W.Mk_localidx (fe_wlocal_offset fe + vloc)) in
+    {| f_locs := <[vloc := v]> (f_locs f);
+       f_inst := f_inst f |}.
+
+  Lemma virt_to_phys_acc ℓ μ a lmask θ ws :
+    let R ns ns32 :=
+      (⌜Forall2 N_i32_repr ns ns32⌝ ∗
+       rt_memaddr sr μ↦[wms][a]flat_map serialise_i32 ns32 ∗
+       words_interp θ μ ws ns)%I in
+    ⊢ rt_token rti sr lmask θ -∗
+      ℓ ↦heap ws -∗
+      ℓ ↦addr (μ, a) -∗
+      ∃ hm,
+        rt_token_nophys rti sr lmask θ hm ∗
+        (∃ ns ns32, R ns ns32) ∗
+        (∀ ns' ns32',
+          R ns' ns32' -∗
+          rt_token_nophys rti sr lmask θ hm -∗
+          ℓ ↦heap ws ∗
+          ℓ ↦addr (μ, a) ∗
+          rt_token rti sr lmask θ).
+  Proof.
+    iIntros (R) "Hrt Hpt Ha".
+    open_rt "Hrt".
+    iExists hm.
+    iCombine "Hpt Hheap" gives "%Hhm".
+    iCombine "Ha Haddr" gives "%Ha".
+    iPoseProof (big_sepM2_lookup_acc with "Hheapmem") as "Hlookup"; eauto.
+    iEval (cbn) in "Hlookup".
+    iSplitL "Hroot Hlayout Hrti Hownmm Howngc Hrootmem"; first by iFrame.
+    iDestruct "Hlookup" as "(HR & Hcont)".
+    iSplitL "HR"; first by iApply "HR".
+    iIntros (ns ns32) "HR Hnp".
+    iPoseProof ("Hcont" with "[$HR]") as "Hclosed".
+    iSplitL "Hpt"; first iFrame.
+    iSplitL "Ha"; first iFrame.
+    iApply (rt_token_putheap with "[$]").
+    iFrame.
+  Qed.
+
+  (* This variant of virt_to_phys_acc does not need an addr points-to and instead expects
+     you to already know θ !! ℓ = Some (MemGC, a). *)
+  Lemma virt_to_phys_acc_gc ℓ a lmask θ ws :
+    let R ns ns32 :=
+      (⌜Forall2 N_i32_repr ns ns32⌝ ∗
+       rt_memaddr sr MemGC↦[wms][a]flat_map serialise_i32 ns32 ∗
+       words_interp θ MemGC ws ns)%I in
+    ⊢ rt_token rti sr lmask θ -∗
+      ℓ ↦heap ws -∗
+      ⌜θ !! ℓ = Some (MemGC, a)⌝ -∗
+      ∃ hm,
+        rt_token_nophys rti sr lmask θ hm ∗
+        (∃ ns ns32, R ns ns32) ∗
+        (∀ ns' ns32',
+          R ns' ns32' -∗
+          rt_token_nophys rti sr lmask θ hm -∗
+          ℓ ↦heap ws ∗
+          rt_token rti sr lmask θ).
+  Proof.
+    iIntros (R) "Hrt Hpt %Ha".
+    open_rt "Hrt".
+    iCombine "Hheap Hpt" gives "%Hpt".
+    iPoseProof (big_sepM2_lookup_acc with "Hheapmem") as "Hlookup"; eauto.
+    iEval (cbn) in "Hlookup".
+    iDestruct "Hlookup" as "(HR & Hcont)".
+    iExists hm.
+    iSplitR "HR Haddr Hheap Hpt Hcont"; first by iFrame.
+    iSplitL "HR"; first by iFrame.
+    iIntros (ns ns32) "HR Htok".
+    iSplitL "Hpt"; first by iFrame.
+    iPoseProof ("Hcont" with "[$HR]") as "Hclosed".
+    iApply (rt_token_putheap with "[$] [$]").
+  Qed.
+
+  Lemma get_path_words1 off ws :
+    off + 1 <= length ws ->
+    ∃ w, get_path_words off 1 ws = [w].
+  Proof.
+    intros Hlen.
+    unfold get_path_words.
+    destruct (drop off ws) as [| w' ws'] eqn:Hdrop;
+      pose proof (f_equal length Hdrop) as Hdroplen;
+      rewrite length_drop in Hdroplen;
+      cbn in Hdroplen.
+    - lia.
+    - eexists; done.
+  Qed.
+
+  Ltac do_get_path_words1 w :=
+     let H := fresh "Hpath" in
+     pose proof (get_path_words1 _ _ ltac:(eauto)) as [w H];
+     rewrite H.
+
+  Lemma get_path_words2 off ws :
+    off + 2 <= length ws ->
+    ∃ w1 w2, get_path_words off 2 ws = [w1; w2].
+  Proof.
+    intros Hlen.
+    unfold get_path_words.
+    destruct (drop off ws) as [| w' [| w'' ws']] eqn:Hdrop;
+      pose proof (f_equal length Hdrop) as Hdroplen;
+      rewrite length_drop in Hdroplen;
+      cbn in Hdroplen;
+      try lia.
+    eexists; eexists; done.
+  Qed.
+
+  Lemma virt_to_phys_slice_acc off sz ℓ μ a lmask θ ws :
+    let slice {A} (x : list A) := take sz (drop off x) in
+    let R ns ns32 :=
+      (⌜Forall2 N_i32_repr ns ns32⌝ ∗
+       rt_memaddr sr μ↦[wms][a + 4 * N.of_nat off]flat_map serialise_i32 ns32 ∗
+       words_interp θ μ (slice ws) ns)%I in
+    ⊢ ⌜off + sz <= length ws⌝ -∗
+      rt_token rti sr lmask θ -∗
+      ℓ ↦heap ws -∗
+      ℓ ↦addr (μ, a) -∗
+      ∃ hm,
+        rt_token_nophys rti sr lmask θ hm ∗
+        (∃ ns ns32, R ns ns32) ∗
+        (∀ ns' ns32',
+          R ns' ns32' -∗
+          rt_token_nophys rti sr lmask θ hm -∗
+          ℓ ↦heap ws ∗
+          ℓ ↦addr (μ, a) ∗
+          rt_token rti sr lmask θ).
+  Proof.
+    iIntros (slice R) "%Hlenbdd Hrt Hpt Ha".
+    open_rt "Hrt".
+    iExists hm.
+    iCombine "Hpt Hheap" gives "%Hhm".
+    iCombine "Ha Haddr" gives "%Ha".
+    iPoseProof (big_sepM2_lookup_acc with "Hheapmem") as "Hlookup"; eauto.
+    iEval (cbn) in "Hlookup".
+    iSplitL "Hroot Hlayout Hrti Hownmm Howngc Hrootmem"; first by iFrame.
+    iDestruct "Hlookup" as "(HR & Hcont)".
+    iDestruct "HR" as "(%ns & %ns32 & %Hns & Hphys & Hwords)".
+    assert (ws = take off ws ++ slice _ ws ++ drop (off + sz) ws) as Hws.
+    {
+      rewrite app_assoc.
+      unfold slice.
+      by rewrite take_take_drop take_drop.
+    }
+    iEval (setoid_rewrite Hws) in "Hwords".
+    iPoseProof (big_sepL2_app_inv_l with "Hwords") as "(%ns_pre & %ns' & -> & Hpre & Hwords)".
+    iPoseProof (big_sepL2_app_inv_l with "Hwords") as "(%ns & %ns_post & -> & Hwords & Hpost)".
+    pose proof Hns as Hns'.
+    apply Forall2_app_inv_l in Hns'.
+    destruct Hns' as (ns32_pre & ns32' & Hns_pre & Hns' & ->).
+    apply Forall2_app_inv_l in Hns'.
+    destruct Hns' as (ns32 & ns32_post & Hns' & Hns_post & ->).
+    rewrite !flat_map_app.
+    rewrite !wms_app; try by eauto.
+    iDestruct "Hphys" as "(Hphys_pre & Hphys & Hphys_post)".
+    pose proof (Forall2_length _ _ _ Hns_pre) as Hnslenpre.
+    pose proof (Forall2_length _ _ _ Hns') as Hnslen.
+    pose proof (Forall2_length _ _ _ Hns_post) as Hnslenpost.
+    iPoseProof (big_sepL2_length with "Hpre") as "%Hlenpre'".
+    iPoseProof (big_sepL2_length with "Hpost") as "%Hlenpost'".
+    iPoseProof (big_sepL2_length with "Hwords") as "%Hlenws'".
+    assert (length (flat_map serialise_i32 ns32_pre) = 4 * off) as Hlenpre.
+    {
+      rewrite len_ser32.
+      rewrite -Hnslenpre -Hlenpre' length_take_le; lia.
+    }
+    rewrite Hlenpre.
+    rewrite Nat2N.inj_mul.
+    iSplitL "Hwords Hphys";
+      first by iFrame.
+    iIntros (ns' ns32') "(%Hns'' & Hphys & Hwords) Hnp".
+    pose proof (Forall2_length _ _ _ Hns'') as Hns32'len.
+    iPoseProof (big_sepL2_length with "Hwords") as "%Hns'len".
+    unfold words_interp.
+    iCombine "Hpre Hwords Hpost" as "Hwords".
+    repeat (rewrite <- big_sepL2_app_same_length; last by intuition congruence).
+    rewrite -Hws.
+    iCombine "Hphys_pre Hphys Hphys_post" as "Hphys".
+    rewrite -wms_app;
+      last by rewrite !len_ser32 -Hns32'len -Hns'len Hlenws' Hnslen.
+    rewrite -wms_app;
+      last (rewrite !len_ser32 -Hnslenpre -Hlenpre' length_take_le; lia).
+    iPoseProof ("Hcont" with "[Hphys Hwords]") as "Hclosed".
+    {
+      rewrite <- !flat_map_app.
+      iFrame.
+      iPureIntro; eauto using Forall2_app.
+    }
+    iSplitL "Hpt"; first iFrame.
+    iSplitL "Ha"; first iFrame.
+    iApply (rt_token_putheap with "[$]").
+    iFrame.
+  Qed.
+
+  Lemma virt_to_phys_slice_acc_gc off sz ℓ μ a lmask θ ws :
+    let slice {A} (x : list A) := take sz (drop off x) in
+    let R ns ns32 :=
+      (⌜Forall2 N_i32_repr ns ns32⌝ ∗
+       rt_memaddr sr μ↦[wms][a + 4 * N.of_nat off]flat_map serialise_i32 ns32 ∗
+       words_interp θ μ (slice ws) ns)%I in
+    ⊢ ⌜off + sz <= length ws⌝ -∗
+      rt_token rti sr lmask θ -∗
+      ℓ ↦heap ws -∗
+      ⌜θ !! ℓ = Some (μ, a)⌝ -∗
+      ∃ hm,
+        rt_token_nophys rti sr lmask θ hm ∗
+        (∃ ns ns32, R ns ns32) ∗
+        (∀ ns' ns32',
+          R ns' ns32' -∗
+          rt_token_nophys rti sr lmask θ hm -∗
+          ℓ ↦heap ws ∗
+          rt_token rti sr lmask θ).
+  Proof.
+    iIntros (slice R) "%Hlenbdd Hrt Hpt %Ha".
+    open_rt "Hrt".
+    iExists hm.
+    iCombine "Hpt Hheap" gives "%Hhm".
+    iPoseProof (big_sepM2_lookup_acc with "Hheapmem") as "Hlookup"; eauto.
+    iEval (cbn) in "Hlookup".
+    iSplitL "Hroot Hlayout Hrti Hownmm Howngc Hrootmem"; first by iFrame.
+    iDestruct "Hlookup" as "(HR & Hcont)".
+    iDestruct "HR" as "(%ns & %ns32 & %Hns & Hphys & Hwords)".
+    assert (ws = take off ws ++ slice _ ws ++ drop (off + sz) ws) as Hws.
+    {
+      rewrite app_assoc.
+      unfold slice.
+      by rewrite take_take_drop take_drop.
+    }
+    iEval (setoid_rewrite Hws) in "Hwords".
+    iPoseProof (big_sepL2_app_inv_l with "Hwords") as "(%ns_pre & %ns' & -> & Hpre & Hwords)".
+    iPoseProof (big_sepL2_app_inv_l with "Hwords") as "(%ns & %ns_post & -> & Hwords & Hpost)".
+    pose proof Hns as Hns'.
+    apply Forall2_app_inv_l in Hns'.
+    destruct Hns' as (ns32_pre & ns32' & Hns_pre & Hns' & ->).
+    apply Forall2_app_inv_l in Hns'.
+    destruct Hns' as (ns32 & ns32_post & Hns' & Hns_post & ->).
+    rewrite !flat_map_app.
+    rewrite !wms_app; try by eauto.
+    iDestruct "Hphys" as "(Hphys_pre & Hphys & Hphys_post)".
+    pose proof (Forall2_length _ _ _ Hns_pre) as Hnslenpre.
+    pose proof (Forall2_length _ _ _ Hns') as Hnslen.
+    pose proof (Forall2_length _ _ _ Hns_post) as Hnslenpost.
+    iPoseProof (big_sepL2_length with "Hpre") as "%Hlenpre'".
+    iPoseProof (big_sepL2_length with "Hpost") as "%Hlenpost'".
+    iPoseProof (big_sepL2_length with "Hwords") as "%Hlenws'".
+    assert (length (flat_map serialise_i32 ns32_pre) = 4 * off) as Hlenpre.
+    {
+      rewrite len_ser32.
+      rewrite -Hnslenpre -Hlenpre' length_take_le; lia.
+    }
+    rewrite Hlenpre.
+    rewrite Nat2N.inj_mul.
+    iSplitL "Hwords Hphys";
+      first by iFrame.
+    iIntros (ns' ns32') "(%Hns'' & Hphys & Hwords) Hnp".
+    pose proof (Forall2_length _ _ _ Hns'') as Hns32'len.
+    iPoseProof (big_sepL2_length with "Hwords") as "%Hns'len".
+    unfold words_interp.
+    iCombine "Hpre Hwords Hpost" as "Hwords".
+    repeat (rewrite <- big_sepL2_app_same_length; last by intuition congruence).
+    rewrite -Hws.
+    iCombine "Hphys_pre Hphys Hphys_post" as "Hphys".
+    rewrite -wms_app;
+      last by rewrite !len_ser32 -Hns32'len -Hns'len Hlenws' Hnslen.
+    rewrite -wms_app;
+      last (rewrite !len_ser32 -Hnslenpre -Hlenpre' length_take_le; lia).
+    iPoseProof ("Hcont" with "[Hphys Hwords]") as "Hclosed".
+    {
+      rewrite <- !flat_map_app.
+      iFrame.
+      iPureIntro; eauto using Forall2_app.
+    }
+    iSplitL "Hpt"; first iFrame.
+    iApply (rt_token_putheap with "[$] [$]").
+  Qed.
+
+  Lemma has_arep_size ι o :
+    has_arep ι o ->
+    length (serialize_atom o) = arep_size ι.
+  Proof.
+    destruct ι, o; intros H; done.
+  Qed.
+
+  Lemma length_t_translate_arep ι :
+    length_t (translate_arep ι) = 4 * arep_size ι.
+  Proof.
+    destruct ι; done.
+  Qed.
+
+  Lemma arep_flags_of_serialize_atom ι o :
+    has_arep ι o →
+    Forall2 word_has_flag (arep_flags ι) (serialize_atom o).
+  Proof.
+    intros Harep. destruct ι, o; try done.
+    all: repeat constructor; done.
+  Qed.
+
+  (* From words_interp, all heap-pointer locations are in dom θ *)
+  Lemma words_interp_locs_dom_θ θ rm μ ws ns :
+    root_ok θ rm →
+    words_interp θ μ ws ns -∗
+    ghost_map_auth rw_root (1/2) rm -∗
+    ⌜Forall (λ ℓ, ℓ ∈ dom θ) (flat_map locations ws)⌝.
+  Proof.
+    iIntros (Hrootok) "Hwords Hroot".
+    iInduction ws as [|w ws'] "IH" forall (ns).
+    - iDestruct (big_sepL2_nil_inv_l with "Hwords") as "->". done.
+    - iDestruct (big_sepL2_cons_inv_l with "Hwords") as "(%n & %ns' & -> & Hword & Hwords')".
+      destruct w as [[m | μ' ℓ] | m].
+      + (* WordPtr (PtrInt m): locations = [] *)
+        iApply ("IH" with "Hwords' Hroot").
+      + (* WordPtr (PtrHeap μ' ℓ): location = [ℓ] *)
+        cbn [flat_map locations].
+        destruct μ, μ'.
+        * (* MemMM / MemMM: word_interp = ⌜repr_pointer θ (PtrHeap MemMM ℓ) n⌝ *)
+          iDestruct "Hword" as "%Hrep".
+          iDestruct ("IH" with "Hwords' Hroot") as "%Htail".
+          iPureIntro. apply Forall_app. split.
+          -- apply Forall_singleton. apply elem_of_dom. inversion Hrep. eauto.
+          -- exact Htail.
+        * (* MemMM / MemGC: word_interp = ∃ a, ⌜repr_root_pointer ...⌝ ∗ a ↦root ℓ *)
+          iDestruct "Hword" as "(%a & _ & Helem)".
+          (* iCombine is non-destructive: Helem and Hroot both remain in context *)
+          iCombine "Helem Hroot" gives "%Hrm".
+          have Hdomℓ : ℓ ∈ dom θ.
+          { apply elem_of_dom.
+            destruct (map_Forall_lookup_1 _ _ _ _ Hrootok Hrm) as [a' Ha']. eauto. }
+          iDestruct ("IH" with "Hwords' Hroot") as "%Htail".
+          iPureIntro. apply Forall_app.
+          by rewrite Forall_singleton.
+        * (* MemGC / MemMM: word_interp = ⌜repr_pointer θ (PtrHeap MemMM ℓ) n⌝ *)
+          iDestruct "Hword" as "%Hrep".
+          iDestruct ("IH" with "Hwords' Hroot") as "%Htail".
+          iPureIntro. apply Forall_app. split.
+          -- apply Forall_singleton. apply elem_of_dom. inversion Hrep. eauto.
+          -- exact Htail.
+        * (* MemGC / MemGC: word_interp = ⌜repr_pointer θ (PtrHeap MemGC ℓ) n⌝ *)
+          iDestruct "Hword" as "%Hrep".
+          iDestruct ("IH" with "Hwords' Hroot") as "%Htail".
+          iPureIntro. apply Forall_app. split.
+          -- apply Forall_singleton. apply elem_of_dom. inversion Hrep. eauto.
+          -- exact Htail.
+      + (* WordInt m: locations = [] *)
+        iApply ("IH" with "Hwords' Hroot").
+  Qed.
+
+  Lemma Forall2_word_has_flag_inj fs1 fs2 ws :
+    Forall2 word_has_flag fs1 ws →
+    Forall2 word_has_flag fs2 ws →
+    fs1 = fs2.
+  Proof.
+    intro H; revert fs2.
+    induction H as [|f1 fs1' w ws' Hf1 _ IH]; intros fs2 H2.
+    - inversion H2; done.
+    - inversion H2 as [|f2 ? ? ? Hf2 H2' Heq1 Heq2]; subst.
+      f_equal.
+      + destruct f1, f2, w; simpl in *; try congruence; by destruct fs1'.
+      + exact (IH _ H2').
+  Qed.
+
+  (* The flag structure is preserved when updating a slice with a same-arep atom.
+     The old slice (take (arep_size ι) (drop off ws)) must already have flags
+     arep_flags ι. *)
+  Lemma update_path_words_flags_compat ι o ws off :
+    has_arep ι o →
+    off + arep_size ι ≤ length ws →
+    Forall2 word_has_flag (arep_flags ι) (take (arep_size ι) (drop off ws)) →
+    ∀ flags, Forall2 word_has_flag flags ws →
+             Forall2 word_has_flag flags (update_path_words off ws (serialize_atom o)).
+  Proof.
+    intros Harep Hbound Holdflags flags Hflags.
+    pose proof (arep_flags_of_serialize_atom ι o Harep) as Hser.
+    pose proof (has_arep_size ι o Harep) as Hser_len.
+    have Hmid : take (arep_size ι) (drop off flags) = arep_flags ι.
+    { apply (Forall2_word_has_flag_inj _ _ (take (arep_size ι) (drop off ws))).
+      - apply Forall2_take. apply Forall2_drop. exact Hflags.
+      - exact Holdflags. }
+    unfold update_path_words. rewrite Hser_len.
+    rewrite <- (take_drop off flags).
+    apply Forall2_app.
+    - apply Forall2_take. exact Hflags.
+    - rewrite <- (take_drop (arep_size ι) (drop off flags)).
+      apply Forall2_app.
+      + rewrite Hmid. exact Hser.
+      + rewrite !drop_drop.
+        rewrite Nat.add_comm.
+        by apply Forall2_drop.
+  Qed.
+
+  Lemma update_path_words_empty_1 off ws_new :
+    update_path_words off [] ws_new = ws_new.
+  Proof.
+    unfold update_path_words.
+    by rewrite take_nil !drop_nil app_nil_r.
+  Qed.
+
+  Lemma update_path_words_empty_2 off ws :
+    update_path_words off ws [] = ws.
+  Proof.
+    unfold update_path_words.
+    simpl.
+    by rewrite drop_0 take_drop.
+  Qed.
+
+
+  Lemma update_path_words_succ off w ws ws_new :
+    update_path_words (S off) (w :: ws) ws_new =
+    w :: update_path_words off ws ws_new.
+  Proof.
+    unfold update_path_words.
+    simpl.
+    done.
+  Qed.
+
+  Lemma update_path_words_first w ws w_new ws_new :
+    update_path_words 0 (w :: ws) (w_new :: ws_new) =
+    w_new :: update_path_words 0 ws ws_new.
+  Proof.
+    unfold update_path_words.
+    simpl.
+    done.
+  Qed.
+
+  Lemma updating_words (off : nat) (adding ws : list word) :
+    off + length adding ≤ length ws →
+    ∃ ws1 ws_old ws2,
+      ws = ws1 ++ ws_old ++ ws2 ∧
+      update_path_words off ws adding = ws1 ++ adding ++ ws2 ∧
+      length ws_old = length adding ∧
+      length ws1 = off.
+  Proof.
+    revert off adding.
+    induction ws as [|w ws IH].
+    - intros off adding Hlens.
+      cbn in Hlens. destruct off; [|lia]. destruct adding; [|cbn in Hlens; lia].
+      exists [], [], []. unfold update_path_words. done.
+    - intros off adding Hlens.
+      destruct off.
+      + destruct adding as [|a adding].
+        * exists [], [], (w :: ws). unfold update_path_words. clear_nils. done.
+        * cbn in Hlens.
+          specialize (IH 0 adding ltac:(lia)) as (ws1 & ws_old & ws2 & Hws & Hset & Hlenold & Hlenws1).
+          assert (ws1 = []) as -> by (destruct ws1; [done | cbn in Hlenws1; lia]).
+          cbn in Hws.
+          exists [], (w :: ws_old), ws2.
+          split; [rewrite Hws; done |].
+          split; [clear_nils; rewrite update_path_words_first Hset; done |].
+          split; [cbn; lia | done].
+      + cbn in Hlens.
+        specialize (IH off adding ltac:(lia)) as (ws1 & ws_old & ws2 & Hws & Hset & Hlenold & Hlenws1).
+        exists (w :: ws1), ws_old, ws2.
+        split; [rewrite Hws; done |].
+        split; [rewrite update_path_words_succ Hset; done |].
+        split; [done | cbn; lia].
+  Qed.
+
+  (* this can be generalized but we get offset >= as1 not often *)
+  Lemma update_path_words_too_long :
+    ∀ as1 off as2,
+      update_path_words (off + length as1) as1 as2 = as1 ++ as2.
+  Proof.
+    intros as1.
+    induction as1 as [|a as1]; intros.
+    - cbn.
+      rewrite update_path_words_empty_1.
+      done.
+    - cbn [length].
+      rewrite Nat.add_succ_r.
+      rewrite update_path_words_succ.
+      rewrite IHas1.
+      done.
+  Qed.
+
+  (* note: may need to add length things but I don't think so *)
+  Lemma update_path_words_in_stages:
+    ∀ ws as1 as2 off,
+    update_path_words off ws (as1 ++ as2) =
+      update_path_words (off + length as1) (update_path_words off ws as1) as2.
+  Proof.
+    intros ws.
+    induction ws as [|w ws]; intros.
+    - rewrite !update_path_words_empty_1.
+      rewrite update_path_words_too_long.
+      done.
+    - destruct off.
+      + destruct as1 as [|a as1].
+        * clear_nils.
+          rewrite update_path_words_empty_2.
+          cbn. done.
+        * change ((a::as1)++as2) with (a::as1++as2).
+          do 2 (rewrite update_path_words_first).
+          rewrite IHws.
+          cbn. done.
+      + do 2 (rewrite update_path_words_succ).
+        rewrite IHws.
+        cbn. done.
+  Qed.
+
+
+  (* Locations in update_path_words are covered if old and new words' locs are *)
+  Lemma update_path_words_locs_incl (dom_set : gset location) ws off ws_new :
+    Forall (λ ℓ, ℓ ∈ dom_set) (flat_map locations ws) →
+    Forall (λ ℓ, ℓ ∈ dom_set) (flat_map locations ws_new) →
+    Forall (λ ℓ, ℓ ∈ dom_set) (flat_map locations (update_path_words off ws ws_new)).
+  Proof.
+    revert off ws_new.
+    induction ws as [| w ws];
+    intros off ws_new Hws Hwsnew.
+    - simpl in Hws.
+      by rewrite update_path_words_empty_1.
+    - destruct ws_new as [|w_new ws_new]; first by rewrite update_path_words_empty_2.
+      simpl in Hws.
+      apply Forall_app in Hws as [Hw Hws].
+      destruct off; last first.
+      + rewrite update_path_words_succ.
+        simpl.
+        rewrite Forall_app.
+        split; first done.
+        by apply IHws.
+      + rewrite update_path_words_first.
+        simpl.
+        rewrite Forall_app.
+        simpl in Hwsnew.
+        apply Forall_app in Hwsnew as [Hwnew Hwsnew].
+        split; first done.
+        by apply IHws.
+  Qed.
+
+  (* changing this. This is one that will PRESERVE THE LAYOUT *)
+  (* so ℓ starts in the mask and will end in the mask *)
+  (* the fact that this passes without lmask ℓ means that it can be in or out *)
+  (* I think. It's a bit suspicious to me ngl. *)
+  Lemma heap_ok_update_weak θ lmask lm hm ℓ ws' flags :
+    layout_ok lmask lm hm ->
+    heap_ok θ hm →
+    lm !! ℓ = Some flags →
+    (lmask ℓ → Forall2 word_has_flag flags ws') →
+    Forall (λ ℓ', ℓ' ∈ dom hm) (flat_map locations ws') →
+    Forall (λ ℓ', ℓ' ∈ dom θ) (flat_map locations ws') →
+    layout_ok lmask lm (<[ℓ := ws']> hm) /\ heap_ok θ (<[ℓ := ws']> hm).
+  Proof.
+    intros Hflags (Hdomhm & Hdomθ) Hlm Hws' Hlocshm Hlocsθ.
+    unfold layout_ok in Hflags.
+    unfold map_Forall2 in Hflags, Hdomθ.
+    unfold map_Forall in Hdomhm.
+    have Hhmℓ : is_Some (hm !! ℓ).
+    { have := Hflags ℓ. rewrite Hlm. intros H. inversion H. eauto. }
+    destruct Hhmℓ as [ws_old Hws_old].
+    have Hθℓ : is_Some (θ !! ℓ).
+    { have := Hdomθ ℓ. rewrite Hws_old. intros H. inversion H. eauto. }
+    destruct Hθℓ as [x Hθℓv].
+    split; [| split].
+    - unfold layout_ok. unfold map_Forall2. intro k.
+      destruct (decide (k = ℓ)) as [->|Hne].
+      + rewrite lookup_insert Hlm decide_True; last done. constructor.
+        intros Hl2.
+        (* is_true vs Is_true ... *)
+        eapply Forall2_impl; [by apply Hws'|].
+        intros f w H.  by rewrite H.
+      + rewrite lookup_insert_ne //.
+    - unfold map_Forall. intros k ws Hk.
+      destruct (decide (k = ℓ)) as [->|Hne].
+      + rewrite lookup_insert decide_True in Hk; last done. injection Hk as <-.
+        eapply Forall_impl; first exact Hlocshm.
+        intros ℓ' Hℓ'. rewrite dom_insert_L. set_solver.
+      + rewrite lookup_insert_ne // in Hk.
+        eapply Forall_impl; first exact (Hdomhm k ws Hk).
+        intros ℓ' Hℓ'. rewrite dom_insert_L. set_solver.
+    - unfold map_Forall2. intro k.
+      destruct (decide (k = ℓ)) as [->|Hne].
+      + rewrite lookup_insert Hθℓv decide_True; last done. constructor. exact Hlocsθ.
+      + rewrite lookup_insert_ne //.
+  Qed.
+
+  (* also weak. and here's where you need to know it's in the mask? I think? *)
+  Lemma rt_token_nophys_insert_heap_weak θ lmask hm ℓ ws ws' :
+    hm !! ℓ = Some ws →
+    (lmask ℓ → ∀ flags, Forall2 word_has_flag flags ws → Forall2 word_has_flag flags ws') →
+    Forall (λ ℓ', ℓ' ∈ dom hm) (flat_map locations ws') →
+    Forall (λ ℓ', ℓ' ∈ dom θ) (flat_map locations ws') →
+    rt_token_nophys rti sr lmask θ hm -∗
+    rt_token_nophys rti sr lmask θ (<[ℓ := ws']> hm).
+  Proof.
+    intros Hhm Hflags_compat Hlocshm Hlocsθ.
+    iIntros "(%rm & %lm & Hroot & Hlayout & Hrti & %Hinj & Hownmm & Howngc & %Hrootok & Hrootmem & %Hheapok)".
+    iExists rm, lm.
+    iFrame "Hroot Hlayout Hrti Howngc Hrootmem".
+    iSplit; first done.
+    iSplit; last (iSplit; first done).
+    - (* own_addr_mm θ (<[ℓ := ws']> hm) *)
+      unfold own_addr_mm.
+      have Hhm' : <[ℓ := ws']> hm = <[ℓ := ws']> (delete ℓ hm).
+      { apply map_eq; intros k; destruct (decide (k = ℓ)) as [->|Hne].
+        - rewrite !lookup_insert. by rewrite !decide_True.
+        - by rewrite !lookup_insert_ne // lookup_delete_ne. }
+      rewrite Hhm'.
+      iEval (rewrite big_sepM_insert_delete).
+      rewrite delete_delete_eq.
+      iSplitL "".
+      * iApply own_addr_mm_trivial_list.
+      * iPoseProof (big_sepM_delete _ hm ℓ ws Hhm with "Hownmm") as "[_ $]".
+    - iPureIntro.
+      have Hmapflags : ∃ flags, lm !! ℓ = Some flags ∧
+                                  (lmask ℓ -> Forall2 word_has_flag flags ws).
+       { destruct Hheapok as (Hcomp1 & _).
+         unfold map_Forall2 in Hcomp1. specialize (Hcomp1 ℓ).
+         rewrite Hhm in Hcomp1. inversion Hcomp1. exists x. split; auto. simpl in H1.
+         intros Hl2. specialize (H1 Hl2).
+         eapply Forall2_impl; first exact H1.
+         intros f w H'. destruct (word_has_flag f w) eqn:H''; first done. by rewrite H'' in H'. }
+      destruct Hmapflags as [flags [Hflm Hwsflags]].
+      destruct Hheapok as [Hlayoutok Hheapok ].
+      eapply heap_ok_update_weak.
+      3: exact Hflm.
+      all: try done.
+      intros Hl.
+      specialize (Hwsflags Hl).
+      exact (Hflags_compat Hl flags Hwsflags).
+  Qed.
+
+  Lemma virt_to_phys_slice_store_acc_weak lmask off sz ℓ μ a θ ws :
+    let slice := take sz (drop off ws) in
+    ⊢ ⌜off + sz <= length ws⌝ -∗
+      rt_token rti sr lmask θ -∗
+      ℓ ↦heap ws -∗
+      ℓ ↦addr (μ, a) -∗
+      ∃ hm,
+        ⌜hm !! ℓ = Some ws⌝ ∗
+        ⌜dom θ = dom hm⌝ ∗
+        ⌜Forall (λ ℓ', ℓ' ∈ dom θ) (flat_map locations ws)⌝ ∗
+        rt_token_nophys rti sr lmask θ hm ∗
+        (∃ (ns : list N) (ns32 : list i32),
+          ⌜Forall2 N_i32_repr ns ns32⌝ ∗
+          rt_memaddr sr μ ↦[wms][a + 4 * N.of_nat off] flat_map serialise_i32 ns32 ∗
+          words_interp θ μ slice ns) ∗
+        (∀ (ws_new : list word) (ns' : list N) (ns32' : list i32),
+          ⌜length ws_new = sz⌝ -∗
+          ⌜Forall2 N_i32_repr ns' ns32'⌝ -∗
+          ⌜∀ flags, Forall2 word_has_flag flags ws →
+                    Forall2 word_has_flag flags (update_path_words off ws ws_new)⌝ -∗
+          ⌜Forall (λ ℓ', ℓ' ∈ dom hm) (flat_map locations (update_path_words off ws ws_new))⌝ -∗
+          ⌜Forall (λ ℓ', ℓ' ∈ dom θ) (flat_map locations (update_path_words off ws ws_new))⌝ -∗
+          rt_memaddr sr μ ↦[wms][a + 4 * N.of_nat off] flat_map serialise_i32 ns32' -∗
+          words_interp θ μ ws_new ns' -∗
+          rt_token_nophys rti sr lmask θ hm -∗
+          |==> ℓ ↦heap (update_path_words off ws ws_new) ∗
+               ℓ ↦addr (μ, a) ∗
+               rt_token rti sr lmask θ).
+  Proof.
+    iIntros (slice) "%Hlenbdd Hrt Hpt Ha".
+    open_rt "Hrt".
+    iExists hm.
+    iCombine "Hpt Hheap" gives "%Hhm".
+    iCombine "Ha Haddr" gives "%Hθℓ".
+    iPoseProof (heap_memory_dom_eq with "Hheapmem") as "%Hdomθhm".
+    iPoseProof (heap_memory_delete _ ℓ _ _ ws with "Hheapmem") as "(HR & Hheapcont)"; eauto.
+    (* Derive Forall (ℓ' ∈ dom θ) (flat_map locations ws) from heap_ok condition 3 *)
+    have Hlocsθ_ws : Forall (λ ℓ', ℓ' ∈ dom θ) (flat_map locations ws).
+    { destruct Hheapok as (_ & Hdomθ).
+      unfold map_Forall2 in Hdomθ.
+      specialize (Hdomθ ℓ).
+      rewrite Hhm Hθℓ in Hdomθ.
+      inversion Hdomθ. exact H1. }
+    iSplit; first (iPureIntro; exact Hhm).
+    iSplit; first (iPureIntro; exact Hdomθhm).
+    iSplit; first (iPureIntro; exact Hlocsθ_ws).
+    iSplitL "Hroot Hlayout Hrti Hownmm Howngc Hrootmem"; first by iFrame.
+    iDestruct "HR" as "(%ns_all & %ns32_all & %Hns_all & Hphys_all & Hwords_all)".
+    assert (ws = take off ws ++ slice ++ drop (off + sz) ws) as Hws.
+    {
+      rewrite app_assoc. unfold slice. by rewrite take_take_drop take_drop.
+    }
+    assert (length slice = sz) as Hslicelen.
+    { unfold slice; apply length_take_le; rewrite length_drop; lia. }
+    iEval (setoid_rewrite Hws) in "Hwords_all".
+    iPoseProof (big_sepL2_app_inv_l with "Hwords_all") as "(%ns_pre & %ns_rest & -> & Hpre & Hwords_rest)".
+    iPoseProof (big_sepL2_app_inv_l with "Hwords_rest") as "(%ns_mid & %ns_post & -> & Hwords & Hpost)".
+    pose proof Hns_all as Hns_all'.
+    apply Forall2_app_inv_l in Hns_all'.
+    destruct Hns_all' as (ns32_pre & ns32_rest & Hns_pre & Hns_rest & ->).
+    apply Forall2_app_inv_l in Hns_rest.
+    destruct Hns_rest as (ns32_mid & ns32_post & Hns_mid & Hns_post & ->).
+    rewrite !flat_map_app.
+    rewrite !wms_app; try by eauto.
+    iDestruct "Hphys_all" as "(Hphys_pre & Hphys & Hphys_post)".
+    pose proof (Forall2_length _ _ _ Hns_pre) as Hnslenpre.
+    pose proof (Forall2_length _ _ _ Hns_mid) as Hnslen.
+    iPoseProof (big_sepL2_length with "Hpre") as "%Hlenpre'".
+    iPoseProof (big_sepL2_length with "Hpost") as "%Hlenpost'".
+    iPoseProof (big_sepL2_length with "Hwords") as "%Hlenws'".
+    assert (length (flat_map serialise_i32 ns32_pre) = 4 * off) as Hlenpre.
+    {
+      rewrite len_ser32. rewrite -Hnslenpre -Hlenpre' length_take_le; lia.
+    }
+    rewrite Hlenpre Nat2N.inj_mul.
+    iSplitL "Hwords Hphys"; first by iFrame.
+    (* Closing frame *)
+    iIntros (ws_new ns' ns32') "%Hlenws_new %Hns'' %Hflags_compat %Hlocshm %Hlocsθ Hphys' Hwords' Hnp".
+    iMod (ghost_map_update (update_path_words off ws ws_new) with "Hheap Hpt") as "[Hheap' Hpt']".
+    iModIntro.
+    iFrame "Hpt' Ha".
+    pose proof (Forall2_length _ _ _ Hns'') as Hns32'len.
+    iPoseProof (big_sepL2_length with "Hwords'") as "%Hns'len".
+    set (hm' := <[ℓ := update_path_words off ws ws_new]> hm).
+    iAssert (rt_token_nophys rti sr lmask θ hm') with "[Hnp]" as "Hnp'".
+    { iApply (rt_token_nophys_insert_heap_weak _ _ _ _ ws with "Hnp").
+      - exact Hhm.
+      - intro Hcontra; done.
+      - eauto.
+      - eauto. }
+    iApply (rt_token_putheap _ _ lmask θ hm' with "Hnp'").
+    unfold rt_token_phys.
+    iFrame "Haddr Hheap'".
+    iApply ("Hheapcont" $! (update_path_words off ws ws_new)).
+    iExists (ns_pre ++ ns' ++ ns_post), (ns32_pre ++ ns32' ++ ns32_post).
+    iSplit; first by (iPureIntro; eauto using Forall2_app).
+    iSplitL "Hphys_pre Hphys' Hphys_post".
+    - iCombine "Hphys_pre Hphys' Hphys_post" as "Hphys_all".
+      rewrite -wms_app; last by (rewrite !len_ser32; lia).
+      rewrite -wms_app; last (rewrite !len_ser32 -Hnslenpre -Hlenpre' length_take_le; lia).
+      rewrite -!flat_map_app.
+      iFrame "Hphys_all".
+    - unfold update_path_words; rewrite Hlenws_new.
+      unfold words_interp.
+      iCombine "Hpre Hwords' Hpost" as "Hwords_all".
+      repeat (rewrite <- big_sepL2_app_same_length; last by (rewrite -?Hlenpre' -?Hns'len; lia)).
+      rewrite drop_drop.
+      iFrame.
+  Qed.
+
+  Lemma atom_to_words_mm θ ι o val_v :
+    has_arep ι o ->
+    atom_interp_weak θ MemMM o val_v -∗
+    ∃ (ns : list N) (ns32 : list i32),
+      ⌜Forall2 N_i32_repr ns ns32⌝ ∗
+      ⌜flat_map serialise_i32 ns32 = bits val_v⌝ ∗
+      ⌜types_agree (translate_arep ι) val_v⌝ ∗
+      words_interp θ MemMM (serialize_atom o) ns.
+  Proof.
+    iIntros (Harep) "Hat".
+    destruct ι.
+    - pose proof Harep as Harepsave.
+      destruct o; cbn in Harep; try inversion Harep; clear Harep.
+      iEval (cbn) in "Hat".
+      iDestruct "Hat" as "(%n & %n32 & %Nrepr & -> & Hat)".
+      iExists [n], [n32].
+      iSplitR; [|iSplitR; [|iSplitR]]; try iPureIntro; try done; try (constructor;done).
+      cbn.
+      iFrame.
+    - destruct o; cbn in Harep; try inversion Harep; clear Harep.
+      iEval (cbn) in "Hat".
+      iDestruct "Hat" as "->".
+      cbn.
+      unfold word_interp.
+      iExists [(Z.to_N (Wasm_int.Int32.unsigned n))].
+      iExists [n].
+      iSplitR; [|iSplitR; [|iSplitR]]; try iPureIntro; try done; try (constructor;done).
+      cbn.
+      auto.
+    - destruct o; cbn in Harep; try inversion Harep; clear Harep.
+      iEval (cbn) in "Hat".
+      iDestruct "Hat" as "->".
+      cbn.
+      unfold word_interp.
+      iExists [(Z.to_N (Wasm_int.Int32.Z_mod_modulus (Wasm_int.Int64.unsigned n)));
+        (Z.to_N (Wasm_int.Int64.unsigned n ≫ 32))].
+      iExists _.
+  (* I'm pretty confident this is true but splitting apart the serializing
+     is tricky? *)
+      admit.
+      (* iSplitR; [|iSplitR; [|iSplitR]]; try iPureIntro; try done; try (constructor;done). *)
+      (* 2: { *)
+      (*   Search serialise_i64. *)
+      (* } *)
+      (* + constructor. *)
+      (*   * Check ((Wasm_int.Int32.Z_mod_modulus (Wasm_int.Int64.unsigned n))). *)
+      (*     Search i64. *)
+      (*     Search (Wasm_int.Int32.Z_mod_modulus). *)
+      (*     instantiate (1:= ((Wasm_int.Int32.Z_mod_modulus (Wasm_int.Int64.unsigned n)))). *)
+      (* auto. *)
+  Admitted.
+
+
+  Lemma atom_to_words_gc θ ι o val_v :
+    has_arep ι o ->
+    atom_interp_weak θ MemGC o val_v -∗
+    ∃ (ns : list N) (ns32 : list i32),
+      ⌜Forall2 N_i32_repr ns ns32⌝ ∗
+      ⌜flat_map serialise_i32 ns32 = bits val_v⌝ ∗
+      ⌜types_agree (translate_arep ι) val_v⌝ ∗
+      words_interp θ MemGC (serialize_atom o) ns.
+  Proof.
+    iIntros (Harep) "Hat".
+    destruct ι.
+    - pose proof Harep as Harepsave.
+      destruct o; cbn in Harep; try inversion Harep; clear Harep.
+      iEval (cbn) in "Hat".
+      iDestruct "Hat" as "(%n & %n32 & %Nrepr & -> & Hat)".
+      iExists [n], [n32].
+      iSplitR; [|iSplitR; [|iSplitR]]; try iPureIntro; try done; try (constructor;done).
+      cbn.
+      iFrame.
+      (* okay cool! I expect the other cases to be as true as the mm ones *)
+    - destruct o; cbn in Harep; try inversion Harep; clear Harep.
+      iEval (cbn) in "Hat".
+      iDestruct "Hat" as "->".
+      cbn.
+      unfold word_interp.
+      iExists [(Z.to_N (Wasm_int.Int32.unsigned n))].
+      iExists [n].
+      iSplitR; [|iSplitR; [|iSplitR]]; try iPureIntro; try done; try (constructor;done).
+      cbn.
+      auto.
+  Admitted.
+
+  Lemma has_areps_size ιs os :
+    Forall2 has_arep ιs os ->
+    map (length ∘ serialize_atom) os = map arep_size ιs.
+  Proof.
+    intros Hall; induction Hall; first done.
+    cbn.
+    erewrite has_arep_size; eauto.
+    congruence.
+  Qed.
+
+  Definition ptr_root
+    (θ : address_map) (μ : base_memory) (o : atom) (v : value) : iProp Σ :=
+    match o with
+    | PtrA p =>
+        ∃ n n32,
+          ⌜N_i32_repr n n32⌝ ∗
+          ⌜v = VAL_int32 n32⌝ ∗
+          match μ, p with
+          | MemMM, PtrHeap MemGC ℓ =>
+              ∃ a, ⌜repr_root_pointer (RootHeap MemGC a) n⌝ ∗ a ↦root ℓ
+          | _, _ => ⌜repr_pointer θ p n⌝
+          end
+    | I32A n => ⌜v = VAL_int32 n⌝
+    | I64A n => ⌜v = VAL_int64 n⌝
+    | F32A n => ⌜v = VAL_float32 n⌝
+    | F64A n => ⌜v = VAL_float64 n⌝
+    end.
+
+
+  (* not the most informative option here. we will want to know that
+     [atom_interp o v] eventually... *)
+  Lemma reconstitute_val θ μ o ws off ι ns ns32 :
+    "Hws" ∷ words_interp θ μ (get_path_words off (arep_size ι) ws) ns -∗
+    "%Hbound" ∷ ⌜off + arep_size ι <= length ws⌝ -∗
+    "%Harep" ∷ ⌜has_arep ι o⌝ -∗
+    "%Hser" ∷ ⌜serialize_atom o = get_path_words off (arep_size ι) ws⌝ -∗
+    "%Hns" ∷ ⌜Forall2 N_i32_repr ns ns32⌝ -∗
+    ∃ v, ⌜flat_map serialise_i32 ns32 = bits v⌝ ∗
+         atom_interp_weak θ μ o v ∗
+         (atom_interp_weak θ μ o v -∗
+          words_interp θ μ (get_path_words off (arep_size ι) ws) ns).
+  Proof.
+    repeat iIntros "@".
+    set (bs := flat_map serialise_i32 ns32).
+    pose proof Hns as Hnslen.
+    pose proof (has_arep_size ι o Harep) as Hreplen.
+    apply Forall2_length in Hnslen.
+    iPoseProof (big_sepL2_length with "Hws") as "%Hlenws".
+    assert (length ns32 = length (get_path_words off (arep_size ι) ws)) as Hseglen;
+      first by rewrite Hlenws.
+    destruct o, ι; try elim Harep.
+    - iExists (wasm_deserialise bs T_i32).
+      iSplitR.
+      {
+        rewrite bits_deserialise; first done.
+        rewrite len_ser32.
+        rewrite Hseglen -Hser.
+        by rewrite Hreplen.
+      }
+      cbn in Hbound.
+      inversion Hser as [Hser'].
+      cbn [arep_size] in *.
+      rewrite -Hser'.
+      rewrite -Hser' in Hlenws.
+      destruct ns as [| n [| n' ns']]; cbn in Hlenws; try lia; clear Hlenws.
+      destruct ns32 as [| n32 [| n32' ns32']]; cbn in Hnslen; try lia; clear Hnslen.
+      inversion Hns as [|A B C D Hn _]; subst A B C D.
+      setoid_rewrite big_sepL2_singleton.
+      destruct μ; [destruct p; [| destruct μ]|];
+        try solve [
+          iDestruct "Hws" as "%Hrep";
+          iPureIntro;
+          intuition;
+          exists n, n32; intuition eauto;
+          cbn [bs flat_map];
+          apply deserialise_serialise_i32
+        ].
+      iDestruct "Hws" as "(%a & %Hrep & Ha)".
+      iSplitL.
+      + iExists n, n32.
+        iFrame.
+        iPureIntro.
+        intuition eauto.
+        apply deserialise_serialise_i32.
+      + iIntros "(%n' & %n32' & %Hrep' & %Hn32' & H'')".
+        rewrite deserialise_serialise_i32 in Hn32'.
+        inversion Hn32'; subst n32'.
+        by rewrite (N_i32_repr_inj n32 n n').
+    - rewrite -Hser.
+      rewrite -Hser in Hlenws; cbn in Hlenws.
+      destruct ns as [| n' [| n'' ns']]; cbn in Hlenws; try lia; clear Hlenws.
+      destruct ns32 as [| n32 [| n32' ns32']]; cbn in Hnslen; try lia; clear Hnslen.
+      inversion Hns as [|A B C D Hn _]; subst A B C D.
+      setoid_rewrite big_sepL2_singleton.
+      iDestruct "Hws" as "%Hws".
+      subst n'.
+      iPureIntro.
+      exists (wasm_deserialise bs T_i32).
+      rewrite bits_deserialise; eauto.
+      intuition.
+      rewrite deserialise_serialise_i32.
+      assert (N_i32_repr (Wasm_int.N_of_uint i32m n) n) by reflexivity.
+      by erewrite (N_i32_repr_inj2 _ n32 n).
+    - rewrite -Hser.
+      rewrite -Hser in Hlenws; cbn in Hlenws.
+      destruct ns as [| n' [| n'' [| n''' ns']]]; cbn in Hlenws; try lia; clear Hlenws.
+      destruct ns32 as [| n32 [| n32' [| n32'' ns32']]]; cbn in Hnslen; try lia; clear Hnslen.
+      inversion Hns as [|A B C D Hn [|A' B' C' D' Hn' _]]; subst.
+      setoid_rewrite big_sepL2_cons.
+      setoid_rewrite big_sepL2_cons.
+      iDestruct "Hws" as "(%Hws1 & %Hws2 & _)".
+      cbn.
+      iPureIntro.
+      exists (wasm_deserialise bs T_i64).
+      intuition.
+      + admit.
+      + admit.
+    - rewrite -Hser.
+      rewrite -Hser in Hlenws; cbn in Hlenws.
+      destruct ns as [| n' [| n'' ns']]; cbn in Hlenws; try lia; clear Hlenws.
+      destruct ns32 as [| n32 [| n32' ns32']]; cbn in Hnslen; try lia; clear Hnslen.
+      inversion Hns as [|A B C D Hn _]; subst A B C D.
+      setoid_rewrite big_sepL2_singleton.
+      iDestruct "Hws" as "%Hws".
+      subst n'.
+      iPureIntro.
+      exists (wasm_deserialise bs T_f32).
+      rewrite bits_deserialise; eauto.
+      intuition.
+      admit. (* need deser-ser lemma *)
+    - rewrite -Hser.
+      rewrite -Hser in Hlenws; cbn in Hlenws.
+      destruct ns as [| n' [| n'' [| n''' ns']]]; cbn in Hlenws; try lia; clear Hlenws.
+      destruct ns32 as [| n32 [| n32' [| n32'' ns32']]]; cbn in Hnslen; try lia; clear Hnslen.
+      inversion Hns as [|A B C D Hn [|A' B' C' D' Hn' _]]; subst.
+      setoid_rewrite big_sepL2_cons.
+      setoid_rewrite big_sepL2_cons.
+      iDestruct "Hws" as "(%Hws1 & %Hws2 & _)".
+      cbn.
+      iPureIntro.
+      exists (wasm_deserialise bs T_f64).
+      intuition.
+      + admit.
+      + admit.
+  Admitted.
+
+  Lemma atom_interp_weak_types_agree ι o μ e v :
+    "%Harep" ∷ ⌜has_arep ι o⌝ -∗
+    "Hat" ∷ atom_interp_weak e μ o v -∗
+     ⌜types_agree (translate_arep ι) v⌝.
+  Proof.
+    repeat iIntros "@".
+    destruct o, ι; try done; cbn [atom_interp_weak];
+      try (iDestruct "Hat" as "->"; done).
+    by iDestruct "Hat" as "(%n & %n32 & _ & -> & _)".
+  Qed.
+
+  Lemma atom_interp_weak_ptr_shaped θ μ p v :
+    atom_interp_weak θ μ (PtrA p) v -∗
+    ⌜∃ n n32, v = VAL_int32 n32 /\ N_i32_repr n n32 /\ ptr_shaped p n⌝.
+  Proof.
+    iIntros "(%n & %n32 & %Hrep & %Heq & H)".
+    subst.
+    iExists n, n32.
+    iSplit; eauto.
+    iSplit; eauto.
+    destruct μ, p; try destruct μ; cbn;
+      try (iDestruct "H" as "%H"; iPureIntro; inversion H; subst; constructor; eauto).
+    iDestruct "H" as "(%a & %repr & _)".
+    iPureIntro.
+    inversion repr; subst; constructor; eauto.
+  Qed.
+
+  Lemma atom_interp_weak_dup θ μ o v :
+    expect_heap_ptr o = None ->
+    Persistent (atom_interp_weak θ μ o v).
+  Proof.
+    intros Heq.
+    unfold atom_interp_weak.
+    destruct o; first destruct p as [n|ℓ], μ;
+      try by inversion Heq;
+      repeat (apply bi.pure_persistent
+      || (apply bi.exist_persistent; intros ?x)
+      || apply bi.sep_persistent).
+  Qed.
+
+  Lemma atom_interp_weak_promote θ μ o v :
+    expect_heap_ptr o = None ->
+    atom_interp_weak θ μ o v -∗
+    atom_interp o v.
+  Proof.
+    intros Heq.
+    unfold atom_interp, atom_interp_weak.
+    destruct o; first destruct p as [n|ℓ] eqn:Hp;
+      try inversion Heq;
+      try (by iIntros "->").
+    destruct μ.
+    all:iIntros "(%n' & %n32 & %Hnrep & -> & %Hrep)".
+    all:cbn.
+    all:iExists _, _; repeat (iSplit; first done).
+    all:iExists (RootInt n).
+    all:cbn.
+    all:inversion Hrep; subst; eauto.
+    all:iPureIntro.
+    all:split; auto.
+    all:by constructor.
+  Qed.
+
+  Lemma heap_ok_update_strong θ lmask lm hm ℓ ws' flags :
+    layout_ok lmask lm hm ->
+    heap_ok θ hm →
+    ¬ lmask ℓ ->
+    lm !! ℓ = Some flags →
+    (* Forall2 word_has_flag flags ws' → *)
+    Forall (λ ℓ', ℓ' ∈ dom hm) (flat_map locations ws') →
+    Forall (λ ℓ', ℓ' ∈ dom θ) (flat_map locations ws') →
+    layout_ok lmask lm (<[ℓ := ws']> hm) /\ heap_ok θ (<[ℓ := ws']> hm).
+  Proof.
+    intros Hflags (Hdomhm & Hdomθ) Hlmask Hlm Hlocshm Hlocsθ.
+    unfold layout_ok in Hflags.
+    unfold map_Forall2 in Hflags, Hdomθ.
+    unfold map_Forall in Hdomhm.
+    have Hhmℓ : is_Some (hm !! ℓ).
+    { have := Hflags ℓ. rewrite Hlm. intros H. inversion H. eauto. }
+    destruct Hhmℓ as [ws_old Hws_old].
+    have Hθℓ : is_Some (θ !! ℓ).
+    { have := Hdomθ ℓ. rewrite Hws_old. intros H. inversion H. eauto. }
+    destruct Hθℓ as [x Hθℓv].
+    split; [| split].
+    - unfold layout_ok. unfold map_Forall2. intro k.
+      destruct (decide (k = ℓ)) as [->|Hne].
+      + rewrite lookup_insert Hlm decide_True; last done. constructor.
+        intros Hl2.
+        by specialize (Hlmask Hl2). (* NOTE: THIS IS WHERE LMASK = FALSE COMES IN *)
+      + rewrite lookup_insert_ne //.
+    - unfold map_Forall. intros k ws Hk.
+      destruct (decide (k = ℓ)) as [->|Hne].
+      + rewrite lookup_insert decide_True in Hk; last done. injection Hk as <-.
+        eapply Forall_impl; first exact Hlocshm.
+        intros ℓ' Hℓ'. rewrite dom_insert_L. set_solver.
+      + rewrite lookup_insert_ne // in Hk.
+        eapply Forall_impl; first exact (Hdomhm k ws Hk).
+        intros ℓ' Hℓ'. rewrite dom_insert_L. set_solver.
+    - unfold map_Forall2. intro k.
+      destruct (decide (k = ℓ)) as [->|Hne].
+      + rewrite lookup_insert Hθℓv decide_True; last done. constructor. exact Hlocsθ.
+      + rewrite lookup_insert_ne //.
+  Qed.
+
+
+
+  Lemma wp_mem_load1_cg_state
+    μ fe con lidx off ι wt wl ret wt' wl' es :
+    run_codegen (memory.load1 mr fe μ con lidx off ι) wt wl = inr (ret, wt', wl', es) ->
+    ret = () ∧ wt' = [] ∧ wl' = [translate_arep ι].
+  Proof.
+    unfold load1.
+    intros Hcompile.
+    inv_cg_bind Hcompile [] ?wt ?wt ?wl ?wl es_get ?es_rest Hget Hcompile.
+    inv_cg_bind Hcompile [] ?wt ?wt ?wl ?wl es_load_w ?es_rest Hload_w Hcompile.
+    inv_cg_bind Hcompile [] ?wt ?wt ?wl ?wl es_wlalloc ?es_rest Hwlalloc Hcompile.
+    inv_cg_bind Hcompile [] ?wt ?wt ?wl ?wl es_save ?es_rest Hsave Hcompile.
+    apply wp_wlalloc in Hwlalloc.
+    destruct Hwlalloc as (Hidx & -> & -> & ->).
+    eapply wp_load_w in Hload_w.
+    destruct Hload_w as (_ & -> & -> & Hload_w).
+    inversion Hidx; subst n.
+    inv_cg_emit Hget; subst.
+    inv_cg_emit Hsave; subst.
+    clear Hretval Hretval0.
+    clear_nils.
+    destruct (atomic_rep_eq_dec ι PtrR); subst.
+    - eapply wp_ite_gc_ptr_ptr_cg_state in Hcompile; eauto.
+      destruct Hcompile as (? & ? & ? & ? & ? & ? & ? & ? & ? & ? & ? & Hdup & -> & ->).
+      inv_cg_ret  H.
+      inv_cg_ret  H0.
+      subst; clear_nils.
+      destruct μ.
+      + destruct con.
+        * pose proof (wp_duproot rti sr mr _ _ _ _ _ _ Hdup) as Hduproot.
+          destruct Hduproot as (_ & -> & -> & _).
+          by destruct ret.
+        * inv_cg_ret Hdup.
+          by destruct ret.
+      + pose proof (wp_registerroot rti sr mr _ _ _ _ _ _ Hdup) as Hregroot.
+        destruct Hregroot as (_ & -> & -> & _).
+        by destruct ret.
+    - apply wp_ite_gc_ptr_nonptr in Hcompile; eauto.
+      inv_cg_ret Hcompile; eauto.
+  Qed.
+
+  Lemma inv_foldlM_nil {A B} (f : A → B → codegen A) (a : A) wt wl a' wt' wl' es :
+    run_codegen (foldlM f a []) wt wl = inr (a', wt', wl', es) ->
+    a' = a /\
+    wt' = [] /\
+    wl' = [] /\
+    es = [].
+  Proof.
+    cbn.
+    intros Heq.
+    by inversion Heq.
+  Qed.
+
+  Lemma inv_foldlM_rcons {A B} (f : A → B → codegen A) (b : B) (bs : list B) (a : A) wt wl a' wt' wl' es :
+    run_codegen (foldlM f a (seq.rcons bs b)) wt wl = inr (a', wt', wl', es) ->
+    ∃ a0 wt_b wt_bs wl_b wl_bs es_b es_bs,
+      run_codegen (foldlM f a bs) wt wl = inr (a0, wt_bs, wl_bs, es_bs) ∧
+      run_codegen (f a0 b) (wt ++ wt_bs) (wl ++ wl_bs) = inr (a', wt_b, wl_b, es_b) /\
+      wt' = wt_bs ++ wt_b ∧
+      wl' = wl_bs ++ wl_b ∧
+      es = es_bs ++ es_b.
+  Proof.
+    intros Hcg.
+    unfold foldlM in Hcg.
+    rewrite seq.foldl_rcons in Hcg.
+    inv_cg_bind Hcg a0 wt_bs wt_b wl_bs wl_b es_bs es_b Hbs Hfb.
+    exists a0. repeat eexists; eauto.
+  Qed.
+
+  Lemma Forall2_rcons_inv_l:
+    ∀ {A B : Type} (P : A → B → Prop) (x : A) (l : list A) (k : list B),
+      Forall2 P (seq.rcons l x) k → ∃ (y : B) (k' : list B), P x y ∧ Forall2 P l k' ∧ k = seq.rcons k' y.
+  Proof using.
+  Admitted.
+
+  Lemma big_sepL2_rcons_inv_l:
+    ∀ {PROP : bi} {A B : Type} (Φ : nat → A → B → PROP) (x1 : A) (l1 : list A) (l2 : list B),
+      ([∗ list] k↦y1;y2 ∈ (seq.rcons l1 x1);l2, Φ k y1 y2)
+      ⊢ ∃ (x2 : B) (l2' : list B),
+          ⌜l2 = seq.rcons l2' x2⌝ ∧ Φ 0 x1 x2 ∗ ([∗ list] k↦y1;y2 ∈ l1;l2', Φ (S k) y1 y2).
+  Proof using.
+  Admitted.
+
+  Lemma big_sepL2_rcons_inv_r :
+    ∀ {PROP: bi} {A B : Type} (Φ : nat → A → B → PROP) (x2 : B) (l1 : list A) (l2 : list B),
+         ([∗ list] k↦y1;y2 ∈ l1;(seq.rcons l2 x2), Φ k y1 y2)
+         ⊢ ∃ (x1 : A) (l1' : list A),
+             ⌜l1 = seq.rcons l1' x1⌝ ∧ Φ 0 x1 x2 ∗ ([∗ list] k↦y1;y2 ∈ l1';l2, Φ (S k) y1 y2).
+  Proof using.
+  Admitted.
+
+  Lemma big_sepL2_rcons :
+    ∀ {PROP : bi} {A B : Type} (Φ : nat → A → B → PROP) (x1 : A) (x2 : B) (l1 : list A) (l2 : list B),
+      ([∗ list] k↦y1;y2 ∈ (seq.rcons l1 x1);(seq.rcons l2 x2), Φ k y1 y2) ⊣⊢ Φ 0 x1 x2 ∗ ([∗ list] k↦y1;y2 ∈ l1;l2, Φ (S k) y1 y2).
+  Proof using.
+  Admitted.
+
+  Lemma foldl_map :
+    ∀ A B (f : A → B) l,
+      seq.map f l = seq.foldl (λ l' a, seq.rcons l' (f a)) [] l.
+  Proof.
+    induction l as [| l x] using seq.last_ind; intros *.
+    - reflexivity.
+    - rewrite seq.foldl_rcons.
+      rewrite seq.map_rcons.
+      congruence.
+  Qed.
+
+  Definition mk_load_frame fe f (wl : wlocal_ctx) (vs : list value) :=
+    let vvs := imap (λ i v, (v, length wl + i)) vs in
+    seq.foldl (λ f '(v, vloc), mk_load1_frame fe f vloc v) f vvs.
+
+  Lemma load1_frame_inst fe f v vloc :
+    f_inst (mk_load1_frame fe f v vloc) = f_inst f.
+  Proof.
+    done.
+  Qed.
+
+  Lemma load1_frame_length fe f v vloc :
+    length (f_locs (mk_load1_frame fe f vloc v)) = length (f_locs f).
+  Proof.
+    by rewrite length_insert.
+  Qed.
+
+  Lemma imap_rcons A B (x : A) (xs : list A) (f: nat -> A -> B) :
+    imap f (seq.rcons xs x) = seq.rcons (imap f xs) (f (length xs) x).
+  Proof.
+    revert f.
+    induction xs; intros f.
+    - done.
+    - cbn.
+      f_equal.
+      by rewrite IHxs.
+  Qed.
+
+  Lemma load_frame_inst fe f wl vs :
+    f_inst (mk_load_frame fe f wl vs) = f_inst f.
+  Proof.
+    induction vs using seq.last_ind; cbn.
+    - tauto.
+    - unfold mk_load_frame.
+      rewrite imap_rcons.
+      rewrite seq.foldl_rcons.
+      rewrite load1_frame_inst.
+      apply IHvs.
+  Qed.
+
+  Lemma load_frame_length fe f wl vs :
+    length (f_locs (mk_load_frame fe f wl vs)) = length (f_locs f).
+  Proof.
+    induction vs using seq.last_ind; cbn.
+    - tauto.
+    - unfold mk_load_frame.
+      by rewrite imap_rcons seq.foldl_rcons load1_frame_length IHvs.
+  Qed.
+
+  Lemma mk_load_frame_stable_part fe f wl vs :
+    ∀ i,
+      i < fe_wlocal_offset fe + length wl  ->
+      f_locs (mk_load_frame fe f wl vs) !! i = f_locs f !! i.
+  Proof.
+    induction vs using seq.last_ind; cbn.
+    - tauto.
+    - unfold mk_load_frame.
+      intros i Hlt.
+      rewrite imap_rcons seq.foldl_rcons.
+      rewrite mk_load1_frame_stable_part; [|lia].
+      by rewrite IHvs.
+  Qed.
+
+  Definition mk_load_post os (vs vs' : list value) : iProp Σ :=
+    (⌜seq.size vs = seq.size vs'⌝ ∗
+    [∗ list] o; '(v, v') ∈ os; (seq.zip vs vs'),
+         (⌜atom_copyable o⌝ -∗ atom_interp o v) ∗
+         atom_interp o v')%I.
+
+  Lemma frame_ext : forall f f',
+    f_inst f = f_inst f' ->
+    f_locs f = f_locs f' ->
+    f = f'.
+  Proof.
+    intros [i l] [i' l']; cbn; congruence.
+  Qed.
+
+  Lemma congeal_rcons ιs ι nss ns vs :
+    congeal_atoms (seq.rcons ιs ι) (seq.rcons nss ns) = Some vs ->
+    exists vs' v, vs = seq.rcons vs' v /\ congeal_atoms ιs nss = Some vs' /\ congeal_atom ι ns = Some v.
+  Proof using.
+  Admitted.
+
+  Lemma ref_flag_atoms_interp_rcons:
+    ∀ (ξ : ref_flag) (o : atom) (os : list atom),
+      ref_flag_atoms_interp ξ (SAtoms (seq.rcons os o)) ↔
+      forall_ptr_atom (ref_flag_ptr_interp ξ) o ∧ ref_flag_atoms_interp ξ (SAtoms os).
+  Proof.
+  Admitted.
+
+  (* Lemma rcons_app {X} : forall (xs : list X) x, *)
+  (*     seq.rcons xs x = xs ++ [x]. *)
+  (* Proof. *)
+  (*   induction xs; intros x. *)
+  (*   - reflexivity. *)
+  (*   - cbn. *)
+  (*     by rewrite IHxs. *)
+  (* Qed. *)
+
+  (* Lemma flat_map_rcons X Y (f : X -> list Y) xs x : *)
+  (*   flat_map f (seq.rcons xs x) = flat_map f xs ++ f x. *)
+  (* Proof. *)
+  (*   revert x. *)
+  (*   induction xs; cbn; intros. *)
+  (*   - by clear_nils. *)
+  (*   - by rewrite -app_assoc IHxs. *)
+  (* Qed. *)
+
+  Lemma mk_frame_rcons fe f wl vs v :
+    mk_load1_frame fe (mk_load_frame fe f wl vs) (length wl + length vs) v =
+      mk_load_frame fe f wl (vs ++ [v]).
+  Proof.
+  Admitted.
+
+  Lemma load_fold_offs_len ιs : ∀ off' offs' off offs,
+    seq.foldl (λ '(off, offs) ι, (off + arep_size ι, seq.rcons offs off)) (off, offs) ιs = (off', offs') ->
+    length offs' = length ιs + length offs.
+  Proof.
+    change @length with @seq.size.
+    induction ιs as [| ιs ι] using seq.last_ind; intros * Hfold.
+    - by inversion Hfold.
+    - rewrite seq.foldl_rcons in Hfold.
+      destruct (seq.foldl _ _ _) as [off0 offs0] eqn:?.
+      inversion Hfold; subst; clear Hfold.
+      eapply IHιs in Heqy.
+      rewrite !seq.size_rcons.
+      lia.
+  Qed.
+
+  Lemma simple_fold_fancy_fold ιs : ∀ off' offs' off offs,
+    seq.foldl (λ '(off, offs) ι, (off + arep_size ι, seq.rcons offs off)) (off, offs) ιs = (off', offs') ->
+    seq.foldl (λ off' ι, off' + arep_size ι) off ιs = off'.
+  Proof.
+  Admitted.
+
+  Lemma simple_fold_sum_list_with ιs : ∀ off,
+    seq.foldl (λ off' ι, off' + arep_size ι) off ιs = off + sum_list_with arep_size ιs.
+  Proof.
+    intros off.
+    apply seq_foldl_sum_list_with.
+  Qed.
+
+  (* Lemma sum_list_with_rcons {X : Type} (f : X -> nat) (x : X) (xs : list X) : *)
+  (*   sum_list_with f (seq.rcons xs x) = f x + sum_list_with f xs. *)
+  (* Proof. *)
+  (* Admitted. *)
+
+  Lemma update_update_wordint ιs off ws ns1 ns2 :
+    update_path_words (seq.foldl (λ off' ι0, off' + arep_size ι0) off ιs)
+      (update_path_words off ws (map WordInt ns1))
+      (map WordInt ns2) =
+      update_path_words off ws (map WordInt (ns1 ++ ns2)).
+  Proof.
+  Admitted.
+
+  Lemma Forall2_rcons_inv_r:
+    ∀ {A B : Type} (P : A → B → Prop) (x : B) (l : list B) (k : list A),
+      Forall2 P k (seq.rcons l x) → ∃ (y : A) (k' : list A), P y x ∧ Forall2 P k' l ∧ k = seq.rcons k' y.
+  Proof.
+  Admitted.
+
+  Lemma Forall2_rcons {A B : Type} (P : A -> B -> Prop) xs x ys y :
+    Forall2 P xs ys ->
+    P x y ->
+    Forall2 P (seq.rcons xs x) (seq.rcons ys y).
+  Proof.
+  Admitted.
+
+  Lemma get_path_split_app ι o os off sz ws :
+    off + sz <= length ws ->
+    has_arep ι o ->
+    get_path_words off sz ws = flat_map serialize_atom os ++ serialize_atom o ->
+    arep_size ι <= sz /\
+    get_path_words off (sz - arep_size ι) ws = flat_map serialize_atom os /\
+    get_path_words (off + sz - arep_size ι) (arep_size ι) ws = serialize_atom o.
+  Proof.
+    intros Hlen Ho Hws.
+    assert (arep_size ι ≤ sz).
+    {
+      apply (f_equal length) in Hws.
+      rewrite length_take length_drop length_app in Hws.
+      erewrite has_arep_size in Hws; eauto.
+      lia.
+    }
+    assert (get_path_words off sz ws =
+              get_path_words off (sz - arep_size ι) ws ++
+              get_path_words (off + sz - arep_size ι) (arep_size ι) ws).
+    {
+      unfold get_path_words.
+      replace (@take word sz) with (@take word ((sz - arep_size ι) + arep_size ι));
+        last (f_equal; lia).
+      rewrite -take_take_drop.
+      rewrite drop_drop.
+      repeat f_equal; lia.
+    }
+    rewrite H0 in Hws.
+    eapply app_inj_1 in Hws; eauto.
+    apply (f_equal length) in Hws.
+    rewrite !length_app in Hws.
+    assert (length (get_path_words (off + sz - arep_size ι) (arep_size ι) ws)
+            = arep_size ι) as Hlast
+        by (rewrite length_take length_drop; lia).
+    rewrite Hlast in Hws.
+    erewrite has_arep_size in Hws; last by eauto.
+    lia.
+  Qed.
+
+  Lemma ser_offsets os : ∀ (off : nat) ntgt ws ιs,
+    off + ntgt <= length ws ->
+    Forall2 has_arep ιs os ->
+    get_path_words off ntgt ws = flat_map serialize_atom os ->
+    Forall2
+      (λ o '(off0, sz), serialize_atom o = get_path_words off0 sz ws)
+      os
+     (seq.zip
+        (seq.foldl (λ '(off', offs) ι, ((off' + arep_size ι)%nat, seq.rcons offs off'))
+                   (off, [])
+                   ιs).2
+        (map arep_size ιs)).
+  Proof.
+    induction os as [|os o] using seq.last_ind; intros * Hlen Hreps Hser.
+    - cbn in Hser.
+      inversion Hreps; subst.
+      econstructor.
+    - apply Forall2_rcons_inv_r in Hreps.
+      destruct Hreps as (ι & ιs' & Ho & Hos & ->).
+      change map with @seq.map.
+      rewrite seq.map_rcons.
+      rewrite seq.foldl_rcons.
+      destruct (seq.foldl
+            (λ '(off', offs) (ι0 : atomic_rep),
+               (off' + arep_size ι0, seq.rcons offs off'))
+            (off, []) ιs') as [off' offs] eqn:Hoffs.
+      pose proof Hoffs as Hoffslen.
+      apply load_fold_offs_len in Hoffslen; cbn in Hoffslen; rewrite Nat.add_0_r in Hoffslen.
+      rewrite flat_map_rcons in Hser.
+      rewrite seq.zip_rcons;
+        last (rewrite seq.size_map; by apply Hoffslen).
+      eapply get_path_split_app in Hser; eauto.
+      destruct Hser as (Hsz & Hseros & Hsero).
+      apply Forall2_rcons.
+      + eapply IHos in Hos; try eapply Hseros; eauto; last lia.
+        by rewrite Hoffs in Hos.
+      + eapply simple_fold_fancy_fold in Hoffs; eauto.
+        rewrite simple_fold_sum_list_with in Hoffs; eauto.
+        rewrite -Hoffs.
+        rewrite -Hsero.
+        f_equal.
+        rewrite sum_list_with_list_sum.
+        erewrite <- has_areps_size; last eauto.
+        rewrite -map_map.
+        apply (f_equal length) in Hseros.
+        rewrite length_take length_drop in Hseros.
+        rewrite flat_map_concat_map length_concat in Hseros.
+        rewrite -Hseros.
+        lia.
+  Qed.
+
+End load_common.
