theories/iris/logrel/load_copy.v
@@ -1,0 +1,947 @@
+From mathcomp Require Import eqtype ssrbool.
+
+From Stdlib Require Import NArith.NArith.
+Require Import RichWasm.util.
+Require Import RichWasm.compiler.memory.
+Require Import RichWasm.iris.numerics.
+Require Import RichWasm.iris.runtime.
+Require Import RichWasm.iris.logrel.instr.typing.common.
+Require Import RichWasm.iris.logrel.case_ptr.
+Require Import RichWasm.iris.logrel.path.
+Require Import RichWasm.iris.logrel.roots.
+Require Import RichWasm.iris.logrel.load_common.
+
+Set Bullet Behavior "Strict Subproofs".
+Set Default Goal Selector "!".
+
+Section load_copy.
+
+  Context `{!logrel_na_invs Σ}.
+  Context `{!wasmG Σ}.
+  Context `{!richwasmG Σ}.
+
+  Variable rti : rt_invariant Σ.
+  Variable sr : store_runtime.
+  Variable mr : module_runtime.
+
+
+  Lemma wp_load1_copy_mm (se : @semantic_env Σ) F lidx off ι wt wl ret wt' wl' es :
+    let fe := fe_of_context F in
+    run_codegen (memory.load1 mr fe MemMM Copy lidx off ι) wt wl = inr (ret, wt', wl', es) ->
+    ∀ f ℓ a32 a o ws s E B R θ lmask Φ,
+    ⊢ "Hf" ∷ ↪[frame] f -∗
+      "Hrun" ∷ ↪[RUN] -∗
+      "Hptr" ∷ ℓ ↦heap ws -∗
+      "Haddr" ∷ ℓ ↦addr (MemMM, a) -∗
+      "Hown"  ∷ na_own logrel_nais E -∗
+      "Htok"  ∷ rt_token rti sr lmask θ -∗
+      "Hregf" ∷ instance_rt_func_interp mr.(mr_func_registerroot) sr.(sr_func_registerroot) (spec_registerroot rti sr) f.(f_inst) -∗
+      "%Hmask" ∷ ⌜↑ns_fun (N.of_nat (sr_func_registerroot sr)) ⊆ E⌝ -∗
+      "%Hbound" ∷ ⌜off + arep_size ι ≤ length ws⌝ -∗
+      "%Harep" ∷ ⌜has_arep ι o⌝ -∗
+      "%Hser" ∷ ⌜serialize_atom o = get_path_words off (arep_size ι) ws⌝ -∗
+      "%Hse" ∷ ⌜sem_env_interp F se⌝ -∗
+      "%Hfsz" ∷ ⌜fe_wlocal_offset fe + length wl + length wl' <= length (f_locs f)⌝ -∗
+      "%Hlidx" ∷ ⌜f_locs f !! localimm lidx = Some (VAL_int32 a32)⌝ -∗
+      "%Hrepa" ∷ ⌜N_i32_repr (tag_address MemMM a) a32⌝ -∗
+      "%Hrepa_mod" ∷ ⌜a `mod` 4 = 0⌝%N -∗
+      "%Hrepa_nz" ∷ ⌜a <> 0⌝%N -∗
+      "%Hrepmem" ∷ ⌜N_nat_repr (sr_mem_mm sr) (rt_memaddr sr MemMM)⌝ -∗
+      "%Hmemmm" ∷ ⌜inst_memory (f_inst f) !! base_mem_idx mr MemMM = Some (sr_mem_mm sr)⌝ -∗
+      "%Hmemgc" ∷ ⌜inst_memory (f_inst f) !! base_mem_idx mr MemGC = Some (sr_mem_gc sr)⌝ -∗
+      "HΦ" ∷
+        (∀ f' vf v,
+           "%Hf'"  ∷ ⌜f' = mk_load1_frame fe f (length wl) vf⌝ -∗
+           "%Hvf"  ∷ ⌜types_agree (translate_arep ι) vf⌝ -∗
+           "Hptr"  ∷ ℓ ↦heap ws -∗
+           "Haddr" ∷ ℓ ↦addr (MemMM, a) -∗
+           "Hown"  ∷ na_own logrel_nais E -∗
+           "Htok"  ∷ rt_token rti sr lmask θ -∗
+           "Hregf" ∷ instance_rt_func_interp mr.(mr_func_registerroot) sr.(sr_func_registerroot) (spec_registerroot rti sr) f.(f_inst) -∗
+           "Ho"    ∷ (⌜atom_copyable o⌝ -∗ atom_interp o v) -∗
+           Φ f' [v]) -∗
+      CWP es @ s; E UNDER B; R {{ Φ }}.
+  Proof.
+    unfold load1.
+    intros Hcompile.
+    inv_cg_bind Hcompile [] ?wt ?wt ?wl ?wl es_get ?es_rest Hget Hcompile.
+    inv_cg_bind Hcompile [] ?wt ?wt ?wl ?wl es_load_w ?es_rest Hload_w Hcompile.
+    inv_cg_bind Hcompile [] ?wt ?wt ?wl ?wl es_wlalloc ?es_rest Hwlalloc Hcompile.
+    inv_cg_bind Hcompile [] ?wt ?wt ?wl ?wl es_save ?es_rest Hsave Hcompile.
+    apply wp_wlalloc in Hwlalloc.
+    destruct Hwlalloc as (Hidx & -> & -> & ->).
+    eapply wp_load_w in Hload_w.
+    destruct Hload_w as (_ & -> & -> & Hload_w).
+    inversion Hidx; subst n; clear Hidx.
+    inv_cg_emit Hget; subst.
+    inv_cg_emit Hsave; subst.
+    clear Hretval Hretval0.
+    clear_nils.
+    intros *.
+    repeat iIntros "@".
+    iApply (cwp_seq with "[Hf Hrun]").
+    {
+      iApply (cwp_local_get with "[] [$] [$]"); eauto.
+      now instantiate (1:= λ f' v', ⌜f' = f /\ v' = [VAL_int32 a32]⌝%I).
+    }
+    iIntros (f' vs') "[-> ->] Hf Hrun".
+    rewrite app_assoc.
+    (* Opening virt resources *)
+    iPoseProof (virt_to_phys_slice_acc rti sr off (arep_size ι) with "[//] [$] [$] [$]")
+      as "(%hm & Hnp & [(%ns & %ns32 & %Hrepns & Hphys & Hwords) Hclose])".
+    (* Opening word_interp *)
+    iPoseProof (reconstitute_val rti sr mr with "[$Hwords] [//] [//] [//] [//]") as "(%v & %Hserws & Hat & Hret)".
+    rewrite !Hserws.
+    set (PHYS := (rt_memaddr sr MemMM↦[wms][a + 4 * N.of_nat off]bits v)%I) in *.
+    iPoseProof (atom_interp_weak_types_agree with "[//] [$Hat]") as "%Htag".
+    iApply (cwp_seq with "[Hf Hrun Hphys]").
+    {
+      iApply (Hload_w with "[$] [$] [$]"); try done.
+      instantiate (1 := λ f' v', (⌜f' = f⌝ ∗ ⌜v' = [v]⌝ ∗ PHYS)%I).
+      eauto.
+    }
+    iIntros (? ?) "(-> & -> & Hphys) Hf Hrun".
+    rewrite app_assoc.
+    set (vloc := localimm (W.Mk_localidx (fe_wlocal_offset (fe_of_context F) + length wl))).
+    set (f' := {| f_locs := <[vloc := v]> (f_locs f);
+                  f_inst := f_inst f |}).
+    iApply (cwp_seq with "[Hf Hrun]").
+    {
+      iApply (cwp_local_tee with "[] [$] [$]").
+      - unfold vloc.
+        cbn in *; lia.
+      - now instantiate (1:= λ f'' v'', ⌜f'' = f' /\ v'' = [v]⌝%I).
+    }
+    iIntros (? ?) "(-> & ->) Hf Hrun".
+    destruct (atomic_rep_eq_dec ι PtrR).
+    - subst ι.
+      destruct o; try (exfalso; tauto).
+      iPoseProof (atom_interp_weak_ptr_shaped with "Hat") as "(%pn & %pn32 & -> & %Hpn32 & %Hshp)".
+      eapply wp_ite_gc_ptr_ptr with (evs:= to_consts [VAL_int32 pn32]) (vs:=[VAL_int32 pn32]) in Hcompile;
+        [|by apply Is_true_true, has_values_to_consts|done|done|done].
+      destruct Hcompile as (?wt & ?wt & ?wt & ?wl & ?wl & ?wl & ?es & ?es & ?es & Hcompile).
+      destruct Hcompile as (Hcg1 & Hcg2 & Hcg3 & Hwt7 & Hwl7 & Hes_rest2).
+      iApply (Hes_rest2 with "[$] [$] []").
+      {
+        iPureIntro; cbn.
+        rewrite list_lookup_insert.
+        rewrite decide_True; auto.
+        split; first done.
+        cbn in Hfsz.
+        subst.
+        rewrite !length_app in Hfsz.
+        eapply Nat.lt_le_trans; last apply Hfsz.
+        lia.
+      }
+      iIntros "!> Hf Hrun".
+      subst wt7 wl7.
+      inv_cg_ret Hcg1.
+      inv_cg_ret Hcg2.
+      clear_nils.
+      inversion Hshp; subst; last destruct μ.
+      + iApply (cwp_val with "[$] [$]"); eauto using has_values_to_consts.
+        iAssert (atom_interp (PtrA (PtrInt n)) (VAL_int32 pn32)) as "Hat'".
+        {
+          subst.
+          iExists (2 * n)%N, pn32.
+          repeat iSplit; try done.
+          iExists (RootInt n).
+          iSplit; eauto.
+          iPureIntro; constructor.
+        }
+        iPoseProof ("Hret" with "Hat") as "Hwords".
+        iAssert (ℓ ↦heap ws ∗ ℓ ↦addr (MemMM, a) ∗ rt_token rti sr lmask θ)%I with "[Hclose Hphys Hwords Hnp]" as "(Hheap & Haddr & Htok)".
+        {
+          unfold PHYS.
+          rewrite -Hserws.
+          iApply ("Hclose" with "[Hphys Hwords] [$]").
+          by iFrame.
+        }
+        subst f'.
+        iApply ("HΦ" with "[//] [//] [$] [$] [$] [$] [$] [-]").
+        by iIntros "_".
+      + iApply (cwp_val with "[$] [$]"); eauto using has_values_to_consts.
+        iPoseProof ("Hret" with "Hat") as "Hwords".
+        iAssert (ℓ ↦heap ws ∗ ℓ ↦addr (MemMM, a) ∗ rt_token rti sr lmask θ)%I with "[Hclose Hphys Hwords Hnp]" as "(Hheap & Haddr & Htok)".
+        {
+          unfold PHYS.
+          rewrite -Hserws.
+          iApply ("Hclose" with "[Hphys Hwords] [$]"); by iFrame.
+        }
+        iApply ("HΦ" with "[//] [//] [$] [$] [$] [$] [$] [-]").
+        by iIntros "Hcontra".
+      + iEval (cbn) in "Hat".
+        iDestruct "Hat" as "(%n & %n32 & %Hn32 & %Hpn32' & (%ar & %Har & Hrt))".
+        pose proof (wp_duproot rti sr mr _ _ _ _ _ _ Hcg3) as Hduproot.
+        destruct Hduproot as (_ & -> & -> & Hduproot).
+        clear Hes_rest2.
+        iDestruct "Hnp" as "(%rm & %lm & Hroot & Hlayout & Hrti & Hinj & Hownmm & Howngc & Hrest)".
+        iDestruct "Hrest" as "(%Hrootok & Hrootmem & Hheapok)".
+        iCombine "Hrt" "Hroot" gives "%Hrm".
+        unfold PHYS.
+        rewrite -Hserws.
+        iApply (Hduproot with "[$] [$] [//] [//] [$] [$] [$]
+                  [Hphys Hclose Hret Hlayout
+                   Hrti Hinj Hownmm Howngc Hheapok] [$] [$]"); eauto.
+        {
+          apply Is_true_true.
+          inversion Hpn32'.
+          eapply has_values_to_consts.
+        }
+        {
+          iIntros "Hrt Hgh Hrm".
+          iPoseProof ("Hret" with "[Hrt]") as "Hwords";
+            first by cbn; iFrame; eauto.
+          unfold rt_token_nophys.
+          iPoseProof ("Hclose" with "[Hphys Hwords]") as "Hclose".
+          {
+            by iFrame.
+          }
+          iPoseProof ("Hclose" with "[-]") as "(Hpt & Hpt' & Htok)"; iFrame; eauto.
+          iAccu.
+        }
+        iIntros (ar' ar'32) "%Hreproot %Hrepar Hrt Htok [Hws Ha] Hinvs Hreg".
+        iApply ("HΦ" with "[//] [//] [$] [$] [$] [$] [$] [-]").
+        iIntros "_".
+        cbn.
+        iExists (tag_address MemGC ar'), ar'32.
+        unfold root_pointer_interp.
+        iSplit; first eauto.
+        iSplit; first eauto.
+        iExists (RootHeap MemGC ar').
+        by iFrame.
+    - eapply wp_ite_gc_ptr_nonptr in Hcompile; last assumption.
+      inv_cg_ret Hcompile; subst.
+      clear_nils.
+      iApply (cwp_val with "[$] [$]"); eauto using has_values_to_consts.
+      unfold has_arep in *.
+      assert (expect_heap_ptr o = None).
+      {
+        by destruct o, ι.
+      }
+      assert (Persistent (atom_interp_weak θ MemMM o v));
+        first by apply atom_interp_weak_dup.
+      iPoseProof "Hat" as "#Hat".
+      iPoseProof ("Hret" with "Hat") as "Hwords".
+      iPoseProof ("Hclose" with "[Hphys Hwords] [$Hnp]") as "(Hws & Ha & Htok)".
+      {
+        unfold PHYS.
+        rewrite -Hserws.
+        by iFrame.
+      }
+      iApply ("HΦ" with "[//] [//] [$] [$] [$] [$] [$] [-]").
+      iIntros "_".
+      iApply atom_interp_weak_promote; auto.
+  Qed.
+
+  Lemma wp_load1_copy_gc (se : @semantic_env Σ) F lidx off ι wt wl ret wt' wl' es :
+    let fe := fe_of_context F in
+    run_codegen (memory.load1 mr fe MemGC Copy lidx off ι) wt wl = inr (ret, wt', wl', es) ->
+    ∀ f ℓ a32 a o ws s E B R θ lmask Φ,
+    ⊢ "Hf" ∷ ↪[frame] f -∗
+      "Hrun" ∷ ↪[RUN] -∗
+      "Hptr" ∷ ℓ ↦heap ws -∗
+      "%Haddr" ∷ ⌜θ !! ℓ = Some (MemGC, a)⌝ -∗
+      "Hown"  ∷ na_own logrel_nais E -∗
+      "Htok"  ∷ rt_token rti sr lmask θ -∗
+      "Hregf" ∷ instance_rt_func_interp mr.(mr_func_registerroot) sr.(sr_func_registerroot) (spec_registerroot rti sr) f.(f_inst) -∗
+      "%Hmask" ∷ ⌜↑ns_fun (N.of_nat (sr_func_registerroot sr)) ⊆ E⌝ -∗
+      "%Hbound" ∷ ⌜off + arep_size ι ≤ length ws⌝ -∗
+      "%Harep" ∷ ⌜has_arep ι o⌝ -∗
+      "%Hser" ∷ ⌜serialize_atom o = get_path_words off (arep_size ι) ws⌝ -∗
+      "%Hse" ∷ ⌜sem_env_interp F se⌝ -∗
+      "%Hfsz" ∷ ⌜fe_wlocal_offset fe + length wl + length wl' <= length (f_locs f)⌝ -∗
+      "%Hlidx" ∷ ⌜f_locs f !! localimm lidx = Some (VAL_int32 a32)⌝ -∗
+      "%Hrepa" ∷ ⌜N_i32_repr (tag_address MemGC a) a32⌝ -∗
+      "%Hrepa_mod" ∷ ⌜a `mod` 4 = 0⌝%N -∗
+      "%Hrepa_nz" ∷ ⌜a <> 0⌝%N -∗
+      "%Hrepmem" ∷ ⌜N_nat_repr (sr_mem_mm sr) (rt_memaddr sr MemMM)⌝ -∗
+      "%Hmemmm" ∷ ⌜inst_memory (f_inst f) !! base_mem_idx mr MemMM = Some (sr_mem_mm sr)⌝ -∗
+      "%Hmemgc" ∷ ⌜inst_memory (f_inst f) !! base_mem_idx mr MemGC = Some (sr_mem_gc sr)⌝ -∗
+      "HΦ" ∷ ▷ (∀ f' vf v,
+           "%Hf'"  ∷ ⌜f' = mk_load1_frame fe f (length wl) vf⌝ -∗
+           "%Hvf"  ∷ ⌜types_agree (translate_arep ι) vf⌝ -∗
+           "Hptr"  ∷ ℓ ↦heap ws -∗
+           "Hown"  ∷ na_own logrel_nais E -∗
+           "Htok"  ∷ rt_token rti sr lmask θ -∗
+           "Hregf" ∷ instance_rt_func_interp mr.(mr_func_registerroot) sr.(sr_func_registerroot) (spec_registerroot rti sr) f.(f_inst) -∗
+           "Ho"    ∷ (⌜atom_copyable o⌝ -∗ atom_interp o v) -∗
+           Φ f' [v]) -∗
+      CWP es @ s; E UNDER B; R {{ Φ }}.
+  Proof.
+    iIntros (fe Hcg).
+    unfold load1.
+    inv_cg_bind Hcg [] ?wt ?wt ?wl ?wl es_get ?es_rest Hget Hcg.
+    inv_cg_bind Hcg [] ?wt ?wt ?wl ?wl es_load_w ?es_rest Hload_w Hcg.
+    inv_cg_bind Hcg [] ?wt ?wt ?wl ?wl es_wlalloc ?es_rest Hwlalloc Hcg.
+    inv_cg_bind Hcg [] ?wt ?wt ?wl ?wl es_save es_if Hsave Hcg.
+    destruct ret.
+    inversion Hget; subst; clear Hget.
+    apply wp_load_w in Hload_w.
+    destruct Hload_w as (_ & -> & -> & Hload_w).
+    apply wp_wlalloc in Hwlalloc.
+    destruct Hwlalloc as (Hidx & -> & -> & ->).
+    inversion Hidx; subst n; clear Hidx.
+    inversion Hsave; subst; clear Hsave.
+    clear_nils.
+    intros *.
+    repeat iIntros "@".
+    iApply (cwp_seq with "[Hf Hrun]").
+    {
+      iApply (cwp_local_get with "[] [$] [$]"); eauto.
+      by instantiate (1 := λ f' v', (⌜f' = f⌝ ∗ ⌜v' = [VAL_int32 a32]⌝)%I).
+    }
+    iIntros (f' vs) "[-> ->] Hf Hr".
+    iEval (rewrite app_assoc).
+    (* Converting virtual resources to physical ones *)
+    iPoseProof ( virt_to_phys_slice_acc_gc rti sr off (arep_size ι) with "[//] [$] [$] [//]")
+      as "(%hm & Hnp & [(%ns & %ns32 & %Hrepns & Hphys & Hwords) Hclose])".
+    (* Opening word_interp *)
+    iPoseProof (reconstitute_val rti sr mr with "[$Hwords] [//] [//] [//] [//]")
+      as "(%v & %Hserws & Hat & Hret)".
+    rewrite !Hserws.
+    set (PHYS := (rt_memaddr sr MemGC↦[wms][a + 4 * N.of_nat off]bits v)%I) in *.
+    iPoseProof (atom_interp_weak_types_agree with "[//] [$Hat]") as "%Htag".
+    iApply (cwp_seq with "[Hf Hr Hphys]").
+    {
+      iApply (Hload_w with "[$] [$] [$]"); try done.
+      instantiate (1 := λ f' v', (⌜f' = f⌝ ∗ ⌜v' = [v]⌝ ∗ PHYS)%I).
+      eauto.
+    }
+    iIntros (? ?) "(-> & -> & Hphys) Hf Hrun".
+    rewrite app_assoc.
+    set (vloc := localimm (W.Mk_localidx (fe_wlocal_offset (fe_of_context F) + length wl))).
+    set (f' := {| f_locs := <[vloc := v]> (f_locs f);
+                  f_inst := f_inst f |}).
+    (* Including HΦ here so we can peel a later off of it. *)
+    iApply (cwp_seq with "[Hf Hrun HΦ]").
+    {
+      iApply (cwp_local_tee with "[HΦ] [$] [$]").
+      - unfold vloc.
+        cbn in *; lia.
+      - iModIntro.
+        instantiate (1:= λ f'' v'', (⌜f'' = f' /\ v'' = [v]⌝ ∗ _)%I).
+        iSplit; first done.
+        iApply "HΦ".
+    }
+    iIntros (? ?) "((-> & ->) & HΦ) Hf Hrun".
+    destruct (atomic_rep_eq_dec ι PtrR).
+    - subst ι.
+      destruct o; try (exfalso; tauto).
+      iPoseProof (atom_interp_weak_ptr_shaped with "Hat") as "(%pn & %pn32 & -> & %Hpn32 & %Hshp)".
+      eapply wp_ite_gc_ptr_ptr with (evs:= to_consts [VAL_int32 pn32]) (vs:=[VAL_int32 pn32]) in Hcg;
+        [|by apply Is_true_true, has_values_to_consts|done|done|done].
+      destruct Hcg as (?wt & ?wt & ?wt & ?wl & ?wl & ?wl & ?es & ?es & ?es & Hcompile).
+      destruct Hcompile as (Hcg1 & Hcg2 & Hcg3 & Hwt7 & Hwl7 & Hes_rest2).
+      iApply (Hes_rest2 with "[$] [$] []").
+      {
+        iPureIntro; cbn.
+        rewrite list_lookup_insert.
+        rewrite decide_True; auto.
+        split; first done.
+        cbn in Hfsz.
+        subst.
+        rewrite !length_app in Hfsz.
+        eapply Nat.lt_le_trans; last apply Hfsz.
+        lia.
+      }
+      iIntros "!> Hf Hrun".
+      subst wt7 wl7.
+      inv_cg_ret Hcg1.
+      inv_cg_ret Hcg2.
+      clear_nils.
+      inversion Hshp; subst; last destruct μ eqn:?.
+      + iApply (cwp_val with "[$] [$]"); eauto using has_values_to_consts.
+        iAssert (atom_interp (PtrA (PtrInt n)) (VAL_int32 pn32)) as "Hat'".
+        {
+          subst.
+          iExists (2 * n)%N, pn32.
+          repeat iSplit; try done.
+          iExists (RootInt n).
+          iSplit; eauto.
+          iPureIntro; constructor.
+        }
+        iPoseProof ("Hret" with "Hat") as "Hwords".
+        iAssert (ℓ ↦heap ws ∗ rt_token rti sr lmask θ)%I with "[Hclose Hphys Hwords Hnp]" as "(Hheap & Htok)".
+        {
+          unfold PHYS.
+          rewrite -Hserws.
+          iApply ("Hclose" with "[Hphys Hwords] [$]").
+          by iFrame.
+        }
+        subst f'.
+        iApply ("HΦ" with "[//] [//] [$] [$] [$] [$] [-]").
+        by iIntros "_".
+      + iApply (cwp_val with "[$] [$]"); eauto using has_values_to_consts.
+        iPoseProof ("Hret" with "Hat") as "Hwords".
+        iAssert (ℓ ↦heap ws ∗ rt_token rti sr lmask θ)%I with "[Hclose Hphys Hwords Hnp]" as "(Hheap & Htok)".
+        {
+          unfold PHYS.
+          rewrite -Hserws.
+          iApply ("Hclose" with "[Hphys Hwords] [$]"); by iFrame.
+        }
+        iApply ("HΦ" with "[//] [//] [$] [$] [$] [$] [-]").
+        by iIntros "Hcontra".
+      + iEval (cbn) in "Hat".
+        iPoseProof "Hat" as "#Hat".
+        iPoseProof "Hat" as "(%n & %n32 & %Hn32 & %Ha & %Hrep)".
+        inversion Hrep; subst.
+        iPoseProof ("Hret" with "Hat") as "Hwords".
+        iAssert (ℓ ↦heap ws ∗ rt_token rti sr lmask θ)%I with "[Hclose Hphys Hwords Hnp]" as "(Hheap & Htok)".
+        {
+          unfold PHYS.
+          rewrite -Hserws.
+          iApply ("Hclose" with "[Hphys Hwords] [$]").
+          by iFrame.
+        }
+        pose proof (wp_registerroot rti sr mr _ _ _ _ _ _ Hcg3) as Hregroot.
+        destruct Hregroot as (_ & -> & -> & Hregroot).
+        inversion Ha; subst pn32.
+        iApply (Hregroot with "[HΦ Hheap] [$] [$] [] [$] [$] [$]"); eauto.
+        {
+          apply Is_true_true.
+          subst.
+          eapply has_values_to_consts.
+        }
+        iIntros (ar' ar'32) "%Hreproot Hrt Htok Hinvs %Har'32 Hfn".
+        iApply ("HΦ" with "[] [] [$] [$Hinvs] [$Htok] [$Hfn] [-] "); eauto.
+        iIntros "_".
+        iExists (tag_address MemGC ar'), ar'32.
+        unfold root_pointer_interp.
+        iSplit; first eauto.
+        iSplit; first eauto.
+        iExists (RootHeap MemGC ar').
+        by iFrame.
+    - eapply wp_ite_gc_ptr_nonptr in Hcg; last assumption.
+      inv_cg_ret Hcg; subst.
+      clear_nils.
+      iApply (cwp_val with "[$] [$]"); eauto using has_values_to_consts.
+      unfold has_arep in *.
+      assert (expect_heap_ptr o = None).
+      {
+        by destruct o, ι.
+      }
+      assert (Persistent (atom_interp_weak θ MemGC o v));
+        first by apply atom_interp_weak_dup.
+      iPoseProof "Hat" as "#Hat".
+      iPoseProof ("Hret" with "Hat") as "Hwords".
+      iPoseProof ("Hclose" with "[Hphys Hwords] [$Hnp]") as "(Hws & Htok)".
+      {
+        unfold PHYS.
+        rewrite -Hserws.
+        by iFrame.
+      }
+      iApply ("HΦ" with "[//] [//] [$] [$] [$] [$] [-]").
+      iIntros "_".
+      iApply atom_interp_weak_promote; auto.
+  Qed.
+
+  Lemma wp_mem_load_copy_mm_inner (se : @semantic_env Σ) F lidx ιs :
+    let fe := fe_of_context F in
+    ∀ off wt wl ret wt' wl' es,
+      run_codegen
+        (foldlM
+           (λ off' ι, load1 mr fe MemMM Copy lidx off' ι;; Monad.ret (off' + arep_size ι))
+           off ιs)
+        wt wl = inr (ret, wt', wl', es) →
+      let offs := snd $ seq.foldl (λ '(off', offs) ι, (off' + arep_size ι, seq.rcons offs off'))
+                    (off, []) ιs in
+      let offs_szs := seq.zip offs (map arep_size ιs) in
+      ret = seq.foldl (λ off' ι, off' + arep_size ι) off ιs ∧
+      wt' = [] ∧
+      wl' = map translate_arep ιs ∧
+      ∀ f ℓ a32 a os ws E B R θ lmask Φ,
+    ⊢ "Hptr" ∷ ℓ ↦heap ws -∗
+      "Haddr" ∷ ℓ ↦addr (MemMM, a) -∗
+      "Hown"  ∷ na_own logrel_nais E -∗
+      "Htok"  ∷ rt_token rti sr lmask θ -∗
+      "Hregf" ∷ instance_rt_func_interp mr.(mr_func_registerroot) sr.(sr_func_registerroot) (spec_registerroot rti sr) f.(f_inst) -∗
+      "%Hmask" ∷ ⌜↑ns_fun (N.of_nat (sr_func_registerroot sr)) ⊆ E⌝ -∗
+      "%Hbound" ∷ ⌜off + sum_list_with arep_size ιs ≤ length ws⌝ -∗
+      "%Harep" ∷ ⌜Forall2 has_arep ιs os⌝ -∗
+      "%Hser" ∷ ⌜Forall2 (λ o '(off, sz), serialize_atom o = get_path_words off sz ws) os offs_szs⌝ -∗
+      "%Hse" ∷ ⌜sem_env_interp F se⌝ -∗
+      "%Hfsz" ∷ ⌜fe_wlocal_offset fe + length wl + length wl' <= length (f_locs f)⌝ -∗
+      "%Hlidx" ∷ ⌜f_locs f !! localimm lidx = Some (VAL_int32 a32)⌝ -∗
+      "%Hlidx_bdd" ∷ ⌜localimm lidx < fe_wlocal_offset fe + length wl⌝ -∗
+      "%Hrepa" ∷ ⌜N_i32_repr (tag_address MemMM a) a32⌝ -∗
+      "%Hrepa_mod" ∷ ⌜a `mod` 4 = 0⌝%N -∗
+      "%Hrepa_nz" ∷ ⌜a <> 0⌝%N -∗
+      "%Hrepmem" ∷ ⌜N_nat_repr (sr_mem_mm sr) (rt_memaddr sr MemMM)⌝ -∗
+      "%Hmemmm" ∷ ⌜inst_memory (f_inst f) !! base_mem_idx mr MemMM = Some (sr_mem_mm sr)⌝ -∗
+      "%Hmemgc" ∷ ⌜inst_memory (f_inst f) !! base_mem_idx mr MemGC = Some (sr_mem_gc sr)⌝ -∗
+      "HΦ" ∷
+        (∀ f' vs vsf,
+           "%Hf'"     ∷ ⌜f' = mk_load_frame fe f wl vsf⌝ -∗
+           "%Hvsf" ∷ ⌜Forall2 (λ ι vf, types_agree (translate_arep ι) vf) ιs vsf⌝ -∗
+           "Hptr"  ∷ ℓ ↦heap ws -∗
+           "Haddr" ∷ ℓ ↦addr (MemMM, a) -∗
+           "Hown"  ∷ na_own logrel_nais E -∗
+           "Htok"  ∷ rt_token rti sr lmask θ -∗
+           "Hregf" ∷ instance_rt_func_interp mr.(mr_func_registerroot) sr.(sr_func_registerroot) (spec_registerroot rti sr) f.(f_inst) -∗
+           "Hos"    ∷ ([∗ list] o;v ∈ os; vs, (⌜atom_copyable o⌝ -∗ atom_interp o v)) -∗
+           Φ f' vs) -∗
+      "Hf" ∷ ↪[frame] f -∗
+      "Hrun" ∷ ↪[RUN] -∗
+      CWP es @ E UNDER B; R {{ Φ }}.
+  Proof.
+    induction ιs as [| ιs ι] using seq.last_ind; intros * Hcg *.
+    - cbn in Hcg.
+      inversion Hcg; subst.
+      split; last split; last split; try done.
+      intros *; repeat iIntros "@".
+      iApply (cwp_nil with "[$] [$]").
+      unfold mk_load_frame.
+      iApply ("HΦ" with "[] [//] [$] [$] [$] [$] [$] []").
+      + done.
+      + inversion Harep.
+        by iApply big_sepL2_nil.
+    - apply inv_foldlM_rcons in Hcg.
+      rewrite seq.foldl_rcons.
+      destruct Hcg as (off_ιs & wt_ι & wt_ιs & wl_ι & wl_ιs & es_ι & es_ιs & Hinit & Hlast).
+      destruct Hlast as (Hlast & -> & -> & ->).
+      inv_cg_bind Hlast a0' wt_bs wt_b wl_bs wl_b es_bs es_b Hbs Hfb.
+      subst.
+      inv_cg_ret Hfb; subst.
+      eapply IHιs in Hinit.
+      clear IHιs.
+      destruct Hinit as (-> & -> & -> & Hinit).
+      pose proof Hbs as Hbs'.
+      eapply (wp_mem_load1_cg_state rti sr mr) in Hbs'.
+      destruct Hbs' as (-> & -> & ->).
+      subst; clear_nils.
+      change map with @seq.map.
+      rewrite seq.map_rcons -seq.cats1 W.cat_app.
+      repeat (split; first by auto).
+      intros *; repeat iIntros "@".
+      (* inverting forall2 where there's an rcons in only one side *)
+      pose proof (Forall2_rcons_inv_l _ _ _ _ Harep) as (o & os' & Ho & Hos' & Hos_eq).
+      rewrite Hos_eq in Hser.
+      pose proof (Forall2_rcons_inv_l _ _ _ _ Hser) as ([off' sz'] & offs_szs' & Hsero & Hseros' & Hoffs_szs_eq).
+      unfold offs_szs in Hoffs_szs_eq.
+      remember (seq.foldl (λ '(off', offs) (ι : atomic_rep), (off' + arep_size ι, seq.rcons offs off')) (
+                    off, []) (seq.rcons ιs ι))
+        as big_fold in *.
+      rewrite seq.foldl_rcons in Heqbig_fold.
+      destruct (seq.foldl (λ '(off', offs) (ι : atomic_rep), (off' + arep_size ι, seq.rcons offs off')) (off, []) ιs)
+        as [off0 offs0] eqn:?Hfold.
+      assert (seq.size offs0 = seq.size ιs).
+      {
+        erewrite load_fold_offs_len; eauto.
+        by rewrite Nat.add_0_r.
+      }
+      iPoseProof (Hinit with "[$] [$] [$] [$] [$]") as "Hinit".
+      clear Hinit.
+      repeat iPoseProof ("Hinit" with "[//]") as "Hinit".
+      iSpecialize ("Hinit" with "[] [//] [] [//] [] [//] [//] [//] [//] [//] [//] [//] [//]");
+      last iSpecialize ("Hinit" with "[]").
+      {
+        iPureIntro.
+        rewrite rcons_app sum_list_with_app in Hbound; cbn in Hbound.
+        lia.
+      }
+      {
+        iPureIntro.
+        cbn.
+        change @map with @seq.map in Hoffs_szs_eq.
+        rewrite /offs Heqbig_fold seq.map_rcons in Hoffs_szs_eq.
+        cbn in Hoffs_szs_eq.
+        rewrite seq.zip_rcons in Hoffs_szs_eq; last by rewrite seq.size_map.
+        pose proof (seq.rcons_inj Hoffs_szs_eq) as Hinv.
+        by inversion Hinv; subst.
+      }
+      {
+        iPureIntro.
+        rewrite length_app in Hfsz.
+        unfold fe in Hfsz.
+        change @seq.map with @map in Hfsz.
+        lia.
+      }
+      {
+        iIntros (f' vs vsf).
+        repeat iIntros "@".
+        (* DEMO: using iAccu to save proof state *)
+        let Q := open_constr:(_ : iProp Σ) in
+          instantiate (1 := (λ f0 vs0, ∃ vsf,
+                              (* stuff to say about f0 and vs0 *)
+                              ⌜f0 = mk_load_frame fe f wl vsf⌝ ∗
+                              ⌜Forall2 (λ (ι : atomic_rep) (vf : value), types_agree (translate_arep ι) vf) ιs vsf⌝ ∗
+                              ([∗ list] o0;v ∈ os';vs0, ⌜atom_copyable o0⌝ -∗ atom_interp o0 v) ∗
+                              rt_token rti sr lmask θ ∗
+                              (* evar for collecting everything else *)
+                              (* make sure nothing that goes in here mentions f', or vs! *)
+                              Q)%I).
+        iExists vsf.
+        iFrame "Hos Htok".
+        iSplit; first done.
+        iSplit; first done.
+        (* accumulates everything in the evar *)
+        iNamedAccu.
+      }
+      iApply (cwp_seq with "[Hinit Hf Hrun]");
+        first iApply ("Hinit" with "[$] [$]").
+      iIntros (f' vs') "(%vsf & -> & %Hvsf & Hos & Htok & @ & @ & @ & @) Hf Hr".
+      iApply cwp_val_app; first eauto using has_values_to_consts.
+      iEval (erewrite <- (load_frame_inst fe f wl vsf)) in "Hregf".
+      pose proof Hfold as Hfold'.
+      apply (simple_fold_fancy_fold rti sr mr) in Hfold'.
+      replace offs with (seq.rcons offs0 off0) in *;
+        last by rewrite /offs Heqbig_fold.
+      iApply (wp_load1_copy_mm with "[$] [$] [$] [$] [$] [$] [$]").
+      all:try eauto || iPureIntro.
+      + rewrite simple_fold_sum_list_with.
+        rewrite sum_list_with_rcons in Hbound.
+        lia.
+      + rewrite Hsero.
+        revert Hoffs_szs_eq.
+        change @map with @seq.map.
+        rewrite seq.map_rcons.
+        rewrite seq.zip_rcons;
+          last by rewrite seq.size_map.
+        intros Heq.
+        apply seq.rcons_inj in Heq.
+        inversion Heq; subst off'.
+        f_equal.
+        symmetry; eapply simple_fold_fancy_fold; eauto.
+      + revert Hfsz.
+        change @seq.map with @map.
+        rewrite length_app load_frame_length; cbn.
+        rewrite length_app.
+        lia.
+      + rewrite mk_load_frame_stable_part; done.
+      + rewrite load_frame_inst.
+        eauto.
+      + rewrite load_frame_inst.
+        eauto.
+      + iIntros (f'' vf v) "@@@@@@@@".
+        unfold fvs_combine.
+        iApply ("HΦ" with "[] [] [$] [$] [$] [$] [Hregf] [Ho Hos]").
+        * iPureIntro.
+          instantiate (1:=vsf ++ [vf]).
+          rewrite Hf'.
+          rewrite -mk_frame_rcons; try eauto.
+          f_equal.
+          rewrite length_app length_map.
+          f_equal.
+          eapply Forall2_length; eapply Hvsf.
+        * iPureIntro; rewrite rcons_app.
+          apply Forall2_app; eauto.
+        * by rewrite load_frame_inst.
+        * rewrite Hos_eq -rcons_app big_sepL2_rcons.
+          iFrame.
+  Qed.
+
+  Lemma wp_mem_load_copy_mm (se : @semantic_env Σ) F lidx ιs :
+    let fe := fe_of_context F in
+    ∀ off wt wl ret wt' wl' es,
+      run_codegen (memory.load mr fe MemMM Copy lidx off ιs) wt wl = inr (ret, wt', wl', es) ->
+      let offs := snd $ seq.foldl (λ '(off', offs) ι, (off' + arep_size ι, seq.rcons offs off'))
+                    (off, []) ιs in
+      let offs_szs := seq.zip offs (map arep_size ιs) in
+      ret = () /\
+      wt' = [] ∧
+      wl' = map translate_arep ιs ∧
+      ∀ f ℓ a32 a os ws E B R θ lmask Φ,
+      ⊢ "Hf" ∷ ↪[frame] f -∗
+        "Hrun" ∷ ↪[RUN] -∗
+        "Hptr" ∷ ℓ ↦heap ws -∗
+        "Haddr" ∷ ℓ ↦addr (MemMM, a) -∗
+        "Hown"  ∷ na_own logrel_nais E -∗
+        "Htok"  ∷ rt_token rti sr lmask θ -∗
+        "Hregf" ∷ instance_rt_func_interp mr.(mr_func_registerroot) sr.(sr_func_registerroot) (spec_registerroot rti sr) f.(f_inst) -∗
+        "%Hmask" ∷ ⌜↑ns_fun (N.of_nat (sr_func_registerroot sr)) ⊆ E⌝ -∗
+        "%Hbound" ∷ ⌜off + sum_list_with arep_size ιs ≤ length ws⌝ -∗
+        "%Harep" ∷ ⌜Forall2 has_arep ιs os⌝ -∗
+        "%Hser" ∷ ⌜Forall2 (λ o '(off, sz), serialize_atom o = get_path_words off sz ws) os offs_szs⌝ -∗
+        "%Hse" ∷ ⌜sem_env_interp F se⌝ -∗
+        "%Hfsz" ∷ ⌜fe_wlocal_offset fe + length wl + length wl' <= length (f_locs f)⌝ -∗
+        "%Hlidx" ∷ ⌜f_locs f !! localimm lidx = Some (VAL_int32 a32)⌝ -∗
+        "%Hlidx_bdd" ∷ ⌜localimm lidx < fe_wlocal_offset fe + length wl⌝ -∗
+        "%Hrepa" ∷ ⌜N_i32_repr (tag_address MemMM a) a32⌝ -∗
+        "%Hrepa_mod" ∷ ⌜a `mod` 4 = 0⌝%N -∗
+        "%Hrepa_nz" ∷ ⌜a <> 0⌝%N -∗
+        "%Hrepmem" ∷ ⌜N_nat_repr (sr_mem_mm sr) (rt_memaddr sr MemMM)⌝ -∗
+        "%Hmemmm" ∷ ⌜inst_memory (f_inst f) !! base_mem_idx mr MemMM = Some (sr_mem_mm sr)⌝ -∗
+        "%Hmemgc" ∷ ⌜inst_memory (f_inst f) !! base_mem_idx mr MemGC = Some (sr_mem_gc sr)⌝ -∗
+        "HΦ" ∷
+          (∀ f' vs vsf,
+             "%Hf'"     ∷ ⌜f' = mk_load_frame fe f wl vsf⌝ -∗
+             "%Hvsf" ∷ ⌜Forall2 (λ ι vf, types_agree (translate_arep ι) vf) ιs vsf⌝ -∗
+             "Hptr"  ∷ ℓ ↦heap ws -∗
+             "Haddr" ∷ ℓ ↦addr (MemMM, a) -∗
+             "Hown"  ∷ na_own logrel_nais E -∗
+             "Htok"  ∷ rt_token rti sr lmask θ -∗
+             "Hregf" ∷ instance_rt_func_interp mr.(mr_func_registerroot) sr.(sr_func_registerroot) (spec_registerroot rti sr) f.(f_inst) -∗
+             "Hos"    ∷ ([∗ list] o;v ∈ os; vs, (⌜atom_copyable o⌝ -∗ atom_interp o v)) -∗
+             Φ f' vs) -∗
+        CWP es @ E UNDER B; R {{ Φ }}.
+  Proof.
+    unfold memory.load.
+    intros * Hcg.
+    apply wp_ignore in Hcg.
+    destruct Hcg as (-> & off' & Hcg).
+    pose proof (wp_mem_load_copy_mm_inner se _ _ _ _ _ _ _ _ _ _ Hcg) as (-> & U & V & W).
+    intuition.
+    repeat iIntros "@".
+    iPoseProof W as "W".
+    by repeat (iSpecialize ("W" with "[$]") || iSpecialize ("W" with "[//]")).
+  Qed.
+
+  Lemma wp_mem_load_copy_gc_inner (se : @semantic_env Σ) F lidx ιs :
+    let fe := fe_of_context F in
+    ∀ off wt wl ret wt' wl' es,
+      run_codegen
+        (foldlM
+           (λ off' ι, load1 mr fe MemGC Copy lidx off' ι;; Monad.ret (off' + arep_size ι))
+           off ιs)
+        wt wl = inr (ret, wt', wl', es) →
+      let offs := snd $ seq.foldl (λ '(off', offs) ι, (off' + arep_size ι, seq.rcons offs off'))
+                    (off, []) ιs in
+      let offs_szs := seq.zip offs (map arep_size ιs) in
+      ret = seq.foldl (λ off' ι, off' + arep_size ι) off ιs ∧
+      wt' = [] ∧
+      wl' = map translate_arep ιs ∧
+      ∀ f ℓ a32 a os ws E B R θ lmask Φ,
+      ⊢ "Hf" ∷ ↪[frame] f -∗
+        "Hrun" ∷ ↪[RUN] -∗
+        "Hptr" ∷ ℓ ↦heap ws -∗
+        "%Haddr" ∷ ⌜θ !! ℓ = Some (MemGC, a)⌝ -∗
+        "Hown"  ∷ na_own logrel_nais E -∗
+        "Htok"  ∷ rt_token rti sr lmask θ -∗
+        "Hregf" ∷ instance_rt_func_interp mr.(mr_func_registerroot) sr.(sr_func_registerroot) (spec_registerroot rti sr) f.(f_inst) -∗
+        "%Hmask" ∷ ⌜↑ns_fun (N.of_nat (sr_func_registerroot sr)) ⊆ E⌝ -∗
+        "%Hbound" ∷ ⌜off + sum_list_with arep_size ιs ≤ length ws⌝ -∗
+        "%Harep" ∷ ⌜Forall2 has_arep ιs os⌝ -∗
+        "%Hser" ∷ ⌜Forall2 (λ o '(off, sz), serialize_atom o = get_path_words off sz ws) os offs_szs⌝ -∗
+        "%Hse" ∷ ⌜sem_env_interp F se⌝ -∗
+        "%Hfsz" ∷ ⌜fe_wlocal_offset fe + length wl + length wl' <= length (f_locs f)⌝ -∗
+        "%Hlidx" ∷ ⌜f_locs f !! localimm lidx = Some (VAL_int32 a32)⌝ -∗
+        "%Hlidx_bdd" ∷ ⌜localimm lidx < fe_wlocal_offset fe + length wl⌝ -∗
+        "%Hrepa" ∷ ⌜N_i32_repr (tag_address MemGC a) a32⌝ -∗
+        "%Hrepa_mod" ∷ ⌜a `mod` 4 = 0⌝%N -∗
+        "%Hrepa_nz" ∷ ⌜a <> 0⌝%N -∗
+        "%Hrepmem" ∷ ⌜N_nat_repr (sr_mem_gc sr) (rt_memaddr sr MemGC)⌝ -∗
+        "%Hmemmm" ∷ ⌜inst_memory (f_inst f) !! base_mem_idx mr MemMM = Some (sr_mem_mm sr)⌝ -∗
+        "%Hmemgc" ∷ ⌜inst_memory (f_inst f) !! base_mem_idx mr MemGC = Some (sr_mem_gc sr)⌝ -∗
+        "HΦ" ∷
+          ▷^(length ιs) (∀ f' vs vsf,
+             "%Hf'"  ∷ ⌜f' = mk_load_frame fe f wl vsf⌝ -∗
+             "%Hvsf" ∷ ⌜Forall2 (λ ι vf, types_agree (translate_arep ι) vf) ιs vsf⌝ -∗
+             "Hptr"  ∷ ℓ ↦heap ws -∗
+             "Hown"  ∷ na_own logrel_nais E -∗
+             "Htok"  ∷ rt_token rti sr lmask θ -∗
+             "Hregf" ∷ instance_rt_func_interp mr.(mr_func_registerroot) sr.(sr_func_registerroot) (spec_registerroot rti sr) f.(f_inst) -∗
+             "Hos"    ∷ ([∗ list] o;v ∈ os; vs, (⌜atom_copyable o⌝ -∗ atom_interp o v)) -∗
+             Φ f' vs) -∗
+        CWP es @ E UNDER B; R {{ Φ }}.
+  Proof.
+    induction ιs as [| ιs ι] using seq.last_ind; intros * Hcg *.
+    - cbn in Hcg.
+      inversion Hcg; subst.
+      split; last split; last split; try done.
+      intros *; repeat iIntros "@".
+      iApply (cwp_nil with "[$] [$]").
+      unfold mk_load_frame.
+      iApply ("HΦ" with "[] [//] [$] [$] [$] [$] []").
+      + done.
+      + inversion Harep.
+        by iApply big_sepL2_nil.
+    - apply inv_foldlM_rcons in Hcg.
+      rewrite seq.foldl_rcons.
+      destruct Hcg as (off_ιs & wt_ι & wt_ιs & wl_ι & wl_ιs & es_ι & es_ιs & Hinit & Hlast).
+      destruct Hlast as (Hlast & -> & -> & ->).
+      inv_cg_bind Hlast a0' wt_bs wt_b wl_bs wl_b es_bs es_b Hbs Hfb.
+      subst.
+      inv_cg_ret Hfb; subst.
+      eapply IHιs in Hinit.
+      clear IHιs.
+      destruct Hinit as (-> & -> & -> & Hinit).
+      pose proof Hbs as Hbs'.
+      eapply (wp_mem_load1_cg_state rti sr mr) in Hbs'.
+      destruct Hbs' as (-> & -> & ->).
+      subst; clear_nils.
+      change map with @seq.map.
+      rewrite seq.map_rcons -seq.cats1 W.cat_app.
+      repeat (split; first by auto).
+      intros *; repeat iIntros "@".
+      (* inverting forall2 where there's an rcons in only one side *)
+      pose proof (Forall2_rcons_inv_l _ _ _ _ Harep) as (o & os' & Ho & Hos' & Hos_eq).
+      rewrite Hos_eq in Hser.
+      pose proof (Forall2_rcons_inv_l _ _ _ _ Hser) as ([off' sz'] & offs_szs' & Hsero & Hseros' & Hoffs_szs_eq).
+      unfold offs_szs in Hoffs_szs_eq.
+      remember (seq.foldl (λ '(off', offs) (ι : atomic_rep), (off' + arep_size ι, seq.rcons offs off')) (
+                    off, []) (seq.rcons ιs ι))
+        as big_fold in *.
+      rewrite seq.foldl_rcons in Heqbig_fold.
+      destruct (seq.foldl (λ '(off', offs) (ι : atomic_rep), (off' + arep_size ι, seq.rcons offs off')) (off, []) ιs)
+        as [off0 offs0] eqn:?Hfold.
+      assert (seq.size offs0 = seq.size ιs).
+      {
+        erewrite load_fold_offs_len; eauto.
+        by rewrite Nat.add_0_r.
+      }
+      iEval (change @length with @seq.size;
+             rewrite seq.size_rcons bi.laterN_later)
+        in "HΦ".
+      iApply (cwp_seq with "[-]").
+      {
+        iPoseProof (Hinit with "[$] [$] [$] [//] [$] [$] [$]") as "Hinit".
+        clear Hinit.
+        repeat iPoseProof ("Hinit" with "[//]") as "Hinit".
+        iSpecialize ("Hinit" with "[] [//] [] [//] [] [//] [//] [//] [//] [//] [//] [//] [//]");
+        last iSpecialize ("Hinit" with "[HΦ]").
+        {
+          iPureIntro.
+          rewrite rcons_app sum_list_with_app in Hbound; cbn in Hbound.
+          lia.
+        }
+        {
+          iPureIntro.
+          cbn.
+          change @map with @seq.map in Hoffs_szs_eq.
+          rewrite /offs Heqbig_fold seq.map_rcons in Hoffs_szs_eq.
+          cbn in Hoffs_szs_eq.
+          rewrite seq.zip_rcons in Hoffs_szs_eq; last by rewrite seq.size_map.
+          pose proof (seq.rcons_inj Hoffs_szs_eq) as Hinv.
+          by inversion Hinv; subst.
+        }
+        {
+          iPureIntro.
+          rewrite length_app in Hfsz.
+          unfold fe in Hfsz.
+          change @seq.map with @map in Hfsz.
+          lia.
+        }
+        {
+          iIntros "!>".
+          iIntros (f' vs vsf).
+          repeat iIntros "@".
+          (* DEMO: using iAccu to save proof state *)
+          let Q := open_constr:(_ : iProp Σ) in
+            instantiate (1 := (λ f0 vs0, ∃ vsf,
+                                (* stuff to say about f0 and vs0 *)
+                                ⌜f0 = mk_load_frame fe f wl vsf⌝ ∗
+                                ⌜Forall2 (λ (ι : atomic_rep) (vf : value), types_agree (translate_arep ι) vf) ιs vsf⌝ ∗
+                                ([∗ list] o0;v ∈ os';vs0, ⌜atom_copyable o0⌝ -∗ atom_interp o0 v) ∗
+                                rt_token rti sr lmask θ ∗
+                                (* evar for collecting everything else *)
+                                (* make sure nothing that goes in here mentions f' or vs! *)
+                                Q)%I).
+          iExists vsf.
+          iFrame "Hos Htok".
+          iSplit; first done.
+          iSplit; first done.
+          (* accumulates everything in the evar *)
+          iNamedAccu.
+        }
+        iApply "Hinit".
+      }
+      iIntros (f' vs') "(%vsf & -> & %Hvsf & Hos & Htok & @ & @ & @) Hf Hr".
+      iApply cwp_val_app; first eauto using has_values_to_consts.
+      iEval (erewrite <- (load_frame_inst fe f wl vsf)) in "Hregf".
+      pose proof Hfold as Hfold'.
+      apply (simple_fold_fancy_fold rti sr mr) in Hfold'.
+      replace offs with (seq.rcons offs0 off0) in *;
+        last by rewrite /offs Heqbig_fold.
+      iApply (wp_load1_copy_gc with "[$] [$] [$] [//] [$] [$] [$]").
+      all:try eauto || iPureIntro.
+      + rewrite simple_fold_sum_list_with.
+        rewrite sum_list_with_rcons in Hbound.
+        lia.
+      + rewrite Hsero.
+        revert Hoffs_szs_eq.
+        change @map with @seq.map.
+        rewrite seq.map_rcons.
+        rewrite seq.zip_rcons;
+          last by rewrite seq.size_map.
+        intros Heq.
+        apply seq.rcons_inj in Heq.
+        inversion Heq; subst off'.
+        f_equal.
+        symmetry; eapply simple_fold_fancy_fold; eauto.
+      + revert Hfsz.
+        change @seq.map with @map.
+        rewrite length_app load_frame_length; cbn.
+        rewrite length_app.
+        lia.
+      + rewrite mk_load_frame_stable_part; done.
+      + rewrite load_frame_inst.
+        eauto.
+      + rewrite load_frame_inst.
+        eauto.
+      + iModIntro.
+        iIntros (f'' vf v).
+        repeat iIntros "@".
+        unfold fvs_combine.
+        rewrite load_frame_inst.
+        iApply ("HΦ" with "[] [] [$] [$] [$] [$] [Ho Hos]").
+        * iPureIntro.
+          instantiate (1:=vsf ++ [vf]).
+          rewrite Hf'.
+          rewrite -mk_frame_rcons; eauto.
+          f_equal.
+          rewrite length_app length_map.
+          f_equal.
+          eapply Forall2_length; eapply Hvsf.
+        * iPureIntro; rewrite rcons_app.
+          apply Forall2_app; eauto.
+        * rewrite Hos_eq -rcons_app big_sepL2_rcons.
+          iFrame.
+  Qed.
+
+  Lemma wp_mem_load_copy_gc (se : @semantic_env Σ) F lidx ιs :
+    let fe := fe_of_context F in
+    ∀ off wt wl ret wt' wl' es,
+      run_codegen (memory.load mr fe MemGC Copy lidx off ιs) wt wl = inr (ret, wt', wl', es) ->
+      let offs := snd $ seq.foldl (λ '(off', offs) ι, (off' + arep_size ι, seq.rcons offs off'))
+                    (off, []) ιs in
+      let offs_szs := seq.zip offs (map arep_size ιs) in
+      ret = () /\
+      wt' = [] ∧
+      wl' = map translate_arep ιs ∧
+      ∀ f ℓ a32 a os ws E B R θ lmask Φ,
+      ⊢ "Hf" ∷ ↪[frame] f -∗
+        "Hrun" ∷ ↪[RUN] -∗
+        "Hptr" ∷ ℓ ↦heap ws -∗
+        "%Haddr" ∷ ⌜θ !! ℓ = Some (MemGC, a)⌝ -∗
+        "Hown"  ∷ na_own logrel_nais E -∗
+        "Htok"  ∷ rt_token rti sr lmask θ -∗
+        "Hregf" ∷ instance_rt_func_interp mr.(mr_func_registerroot) sr.(sr_func_registerroot) (spec_registerroot rti sr) f.(f_inst) -∗
+        "%Hmask" ∷ ⌜↑ns_fun (N.of_nat (sr_func_registerroot sr)) ⊆ E⌝ -∗
+        "%Hbound" ∷ ⌜off + sum_list_with arep_size ιs ≤ length ws⌝ -∗
+        "%Harep" ∷ ⌜Forall2 has_arep ιs os⌝ -∗
+        "%Hser" ∷ ⌜Forall2 (λ o '(off, sz), serialize_atom o = get_path_words off sz ws) os offs_szs⌝ -∗
+        "%Hse" ∷ ⌜sem_env_interp F se⌝ -∗
+        "%Hfsz" ∷ ⌜fe_wlocal_offset fe + length wl + length wl' <= length (f_locs f)⌝ -∗
+        "%Hlidx" ∷ ⌜f_locs f !! localimm lidx = Some (VAL_int32 a32)⌝ -∗
+        "%Hlidx_bdd" ∷ ⌜localimm lidx < fe_wlocal_offset fe + length wl⌝ -∗
+        "%Hrepa" ∷ ⌜N_i32_repr (tag_address MemGC a) a32⌝ -∗
+        "%Hrepa_mod" ∷ ⌜a `mod` 4 = 0⌝%N -∗
+        "%Hrepa_nz" ∷ ⌜a <> 0⌝%N -∗
+        "%Hrepmem" ∷ ⌜N_nat_repr (sr_mem_gc sr) (rt_memaddr sr MemGC)⌝ -∗
+        "%Hmemmm" ∷ ⌜inst_memory (f_inst f) !! base_mem_idx mr MemMM = Some (sr_mem_mm sr)⌝ -∗
+        "%Hmemgc" ∷ ⌜inst_memory (f_inst f) !! base_mem_idx mr MemGC = Some (sr_mem_gc sr)⌝ -∗
+        "HΦ" ∷
+          ▷^(length ιs) (∀ f' vs vsf,
+             "%Hf'"  ∷ ⌜f' = mk_load_frame fe f wl vsf⌝ -∗
+             "%Hvsf" ∷ ⌜Forall2 (λ ι vf, types_agree (translate_arep ι) vf) ιs vsf⌝ -∗
+             "Hptr"  ∷ ℓ ↦heap ws -∗
+             "Hown"  ∷ na_own logrel_nais E -∗
+             "Htok"  ∷ rt_token rti sr lmask θ -∗
+             "Hregf" ∷ instance_rt_func_interp mr.(mr_func_registerroot) sr.(sr_func_registerroot) (spec_registerroot rti sr) f.(f_inst) -∗
+             "Hos"    ∷ ([∗ list] o;v ∈ os; vs, (⌜atom_copyable o⌝ -∗ atom_interp o v)) -∗
+             Φ f' vs) -∗
+        CWP es @ E UNDER B; R {{ Φ }}.
+  Proof.
+    intros * Hcg ? ?.
+    apply wp_ignore in Hcg.
+    destruct Hcg as (-> & res' & Hcg).
+    eapply wp_mem_load_copy_gc_inner in Hcg.
+    destruct Hcg as (-> & -> & -> & Hspec).
+    split; first done.
+    split; first done.
+    split; first done.
+    exact Hspec.
+  Qed.
+
+End load_copy.
