theories/iris/logrel/load_move.v
@@ -1,0 +1,355 @@
+From mathcomp Require Import eqtype ssrbool.
+
+From Stdlib Require Import NArith.NArith.
+Require Import RichWasm.util.
+Require Import RichWasm.compiler.memory.
+Require Import RichWasm.iris.numerics.
+Require Import RichWasm.iris.runtime.
+Require Import RichWasm.iris.logrel.instr.typing.common.
+Require Import RichWasm.iris.logrel.case_ptr.
+Require Import RichWasm.iris.logrel.path.
+Require Import RichWasm.iris.logrel.roots.
+Require Import RichWasm.iris.logrel.load_common.
+Require Import RichWasm.iris.logrel.virt_to_phys_strong.
+
+Set Bullet Behavior "Strict Subproofs".
+Set Default Goal Selector "!".
+
+Section load_move.
+
+  Context `{!logrel_na_invs Σ}.
+  Context `{!wasmG Σ}.
+  Context `{!richwasmG Σ}.
+
+  Variable rti : rt_invariant Σ.
+  Variable sr : store_runtime.
+  Variable mr : module_runtime.
+
+  Lemma wp_load1_move_mm (se : @semantic_env Σ) F lidx off ι wt wl ret wt' wl' es :
+    let fe := fe_of_context F in
+    run_codegen (memory.load1 mr fe MemMM Move lidx off ι) wt wl = inr (ret, wt', wl', es) ->
+    ∀ f ℓ a32 a o ws s E B R θ lmask Φ,
+    ⊢ "Hf" ∷ ↪[frame] f -∗
+      "Hrun" ∷ ↪[RUN] -∗
+      "Hptr" ∷ ℓ ↦heap ws -∗
+      "Haddr" ∷ ℓ ↦addr (MemMM, a) -∗
+      "Hown"  ∷ na_own logrel_nais E -∗
+      "Htok"  ∷ rt_token rti sr lmask θ -∗
+      "Hregf" ∷ instance_rt_func_interp mr.(mr_func_registerroot) sr.(sr_func_registerroot) (spec_registerroot rti sr) f.(f_inst) -∗
+      "%Hℓmask"  ∷ ⌜¬ lmask ℓ⌝ -∗
+      "%Hmask" ∷ ⌜↑ns_fun (N.of_nat (sr_func_registerroot sr)) ⊆ E⌝ -∗
+      "%Hbound" ∷ ⌜off + arep_size ι ≤ length ws⌝ -∗
+      "%Harep" ∷ ⌜has_arep ι o⌝ -∗
+      "%Hser" ∷ ⌜serialize_atom o = get_path_words off (arep_size ι) ws⌝ -∗
+      "%Hse" ∷ ⌜sem_env_interp F se⌝ -∗
+      "%Hfsz" ∷ ⌜fe_wlocal_offset fe + length wl + length wl' <= length (f_locs f)⌝ -∗
+      "%Hlidx" ∷ ⌜f_locs f !! localimm lidx = Some (VAL_int32 a32)⌝ -∗
+      "%Hrepa" ∷ ⌜N_i32_repr (tag_address MemMM a) a32⌝ -∗
+      "%Hrepa_mod" ∷ ⌜a `mod` 4 = 0⌝%N -∗
+      "%Hrepa_nz" ∷ ⌜a ≠ 0⌝%N -∗
+      "%Hrepmem" ∷ ⌜N_nat_repr (sr_mem_mm sr) (rt_memaddr sr MemMM)⌝ -∗
+      "%Hmemmm" ∷ ⌜inst_memory (f_inst f) !! base_mem_idx mr MemMM = Some (sr_mem_mm sr)⌝ -∗
+      "%Hmemgc" ∷ ⌜inst_memory (f_inst f) !! base_mem_idx mr MemGC = Some (sr_mem_gc sr)⌝ -∗
+      "HΦ" ∷
+        (∀ f' vf v ns',
+           "%Hns'" ∷ ⌜length ns' = arep_size ι⌝ -∗
+           "%Hf'"  ∷ ⌜f' = mk_load1_frame fe f (length wl) vf⌝ -∗
+           "%Hvf"  ∷ ⌜types_agree (translate_arep ι) vf⌝ -∗
+           "Hptr"  ∷ ℓ ↦heap update_path_words off ws (map WordInt ns') -∗
+           "Haddr" ∷ ℓ ↦addr (MemMM, a) -∗
+           "Hown"  ∷ na_own logrel_nais E -∗
+           "Htok"  ∷ rt_token rti sr lmask θ -∗
+           "Hregf" ∷ instance_rt_func_interp mr.(mr_func_registerroot) sr.(sr_func_registerroot) (spec_registerroot rti sr) f.(f_inst) -∗
+           "Ho"    ∷ atom_interp o v -∗
+           Φ f' [v]) -∗
+      CWP es @ s; E UNDER B; R {{ Φ }}.
+  Proof.
+    unfold load1.
+    intros Hcompile.
+    inv_cg_bind Hcompile [] ?wt ?wt ?wl ?wl es_get ?es_rest Hget Hcompile.
+    inv_cg_bind Hcompile [] ?wt ?wt ?wl ?wl es_load_w ?es_rest Hload_w Hcompile.
+    inv_cg_bind Hcompile [] ?wt ?wt ?wl ?wl es_wlalloc ?es_rest Hwlalloc Hcompile.
+    inv_cg_bind Hcompile [] ?wt ?wt ?wl ?wl es_save ?es_rest Hsave Hcompile.
+    apply wp_wlalloc in Hwlalloc.
+    destruct Hwlalloc as (Hidx & -> & -> & ->).
+    eapply wp_load_w in Hload_w.
+    destruct Hload_w as (_ & -> & -> & Hload_w).
+    inversion Hidx; subst n; clear Hidx.
+    inv_cg_emit Hget; subst.
+    inv_cg_emit Hsave; subst.
+    clear Hretval Hretval0.
+    clear_nils.
+    intros *.
+    repeat iIntros "@".
+    iApply (cwp_seq with "[Hf Hrun]").
+    {
+      iApply (cwp_local_get with "[] [$] [$]"); eauto.
+      now instantiate (1:= λ f' v', ⌜f' = f /\ v' = [VAL_int32 a32]⌝%I).
+    }
+    iIntros (f' vs') "[-> ->] Hf Hrun".
+    rewrite app_assoc.
+    (* Opening virt resources *)
+    iPoseProof (virt_to_phys_slice_store_acc_strong _ _ lmask off (arep_size ι) with "[//] [$] [$] [$] [//]")
+      as "(%hm & %Hhm & %Hdomθhm & %Hlocsθ_ws & Hnp & (%ns & %ns32 & %Hns & Hphys & Hwords) & Hclose)".
+    (* Opening word_interp *)
+    iPoseProof (reconstitute_val rti sr mr with "[$Hwords] [//] [//] [//] [//]") as "(%v & %Hserws & Hat & Hret)".
+    rewrite !Hserws.
+    set (PHYS := (rt_memaddr sr MemMM↦[wms][a + 4 * N.of_nat off]bits v)%I) in *.
+    iPoseProof (atom_interp_weak_types_agree with "[//] [$Hat]") as "%Htag".
+    iApply (cwp_seq with "[Hf Hrun Hphys]").
+    {
+      iApply (Hload_w with "[$] [$] [$]"); try done.
+      instantiate (1 := λ f' v', (⌜f' = f⌝ ∗ ⌜v' = [v]⌝ ∗ PHYS)%I).
+      eauto.
+    }
+    iIntros (? ?) "(-> & -> & Hphys) Hf Hrun".
+    rewrite app_assoc.
+    set (vloc := localimm (W.Mk_localidx (fe_wlocal_offset (fe_of_context F) + length wl))).
+    set (f' := {| f_locs := <[vloc := v]> (f_locs f);
+                  f_inst := f_inst f |}).
+    iApply (cwp_seq with "[Hf Hrun]").
+    {
+      iApply (cwp_local_tee with "[] [$] [$]").
+      - unfold vloc.
+        cbn in *; lia.
+      - now instantiate (1:= λ f'' v'', ⌜f'' = f' /\ v'' = [v]⌝%I).
+    }
+    iIntros (? ?) "(-> & ->) Hf Hrun".
+    iAssert ((CWP es_rest2 @ s; E UNDER B; R {{ f'; vs', ⌜f' = f⌝ ∗ ⌜vs' = []⌝ }})%I) as "Hrest2".
+    {
+      iEval (change es_rest2 with ([] ++ es_rest2)).
+      destruct (atomic_rep_eq_dec ι PtrR); try subst ι.
+      - admit.
+  Admitted.
+
+
+  Lemma wp_mem_load_move_inner ιs :
+    ∀ (se : @semantic_env Σ) F lidx off wt wl ret wt' wl' es,
+    let fe := fe_of_context F in
+      run_codegen
+        (foldlM
+           (λ off' ι, load1 mr fe MemMM Move lidx off' ι;; Monad.ret (off' + arep_size ι))
+           off ιs)
+        wt wl = inr (ret, wt', wl', es) →
+    let offs := snd $ seq.foldl (λ '(off', offs) ι, (off' + arep_size ι, seq.rcons offs off'))
+                  (off, []) ιs in
+    let offs_szs := seq.zip offs (map arep_size ιs) in
+    ret = seq.foldl (λ off' ι, off' + arep_size ι) off ιs ∧
+    wt' = [] ∧
+    wl' = map translate_arep ιs ∧
+    ∀ f ℓ a32 a os ws E B R θ lmask Φ,
+    ⊢ "Hf" ∷ ↪[frame] f -∗
+      "Hrun" ∷ ↪[RUN] -∗
+      "Hptr" ∷ ℓ ↦heap ws -∗
+      "Haddr" ∷ ℓ ↦addr (MemMM, a) -∗
+      "%Hℓmask"  ∷ ⌜¬ lmask ℓ⌝ -∗
+      "Hown"  ∷ na_own logrel_nais E -∗
+      "Htok"  ∷ rt_token rti sr lmask θ -∗
+      "Hregf" ∷ instance_rt_func_interp mr.(mr_func_registerroot) sr.(sr_func_registerroot) (spec_registerroot rti sr) f.(f_inst) -∗
+      "%Hmask" ∷ ⌜↑ns_fun (N.of_nat (sr_func_registerroot sr)) ⊆ E⌝ -∗
+      "%Hbound" ∷ ⌜off + sum_list_with arep_size ιs ≤ length ws⌝ -∗
+      "%Harep" ∷ ⌜Forall2 has_arep ιs os⌝ -∗
+      "%Hser" ∷ ⌜Forall2 (λ o '(off, sz), serialize_atom o = get_path_words off sz ws) os offs_szs⌝ -∗
+      "%Hse" ∷ ⌜sem_env_interp F se⌝ -∗
+      "%Hfsz" ∷ ⌜fe_wlocal_offset fe + length wl + length wl' <= length (f_locs f)⌝ -∗
+      "%Hlidx" ∷ ⌜f_locs f !! localimm lidx = Some (VAL_int32 a32)⌝ -∗
+      "%Hlidx_bdd" ∷ ⌜localimm lidx < fe_wlocal_offset fe + length wl⌝ -∗
+      "%Hrepa" ∷ ⌜N_i32_repr (tag_address MemMM a) a32⌝ -∗
+      "%Hrepa_mod" ∷ ⌜a `mod` 4 = 0⌝%N -∗
+      "%Hrepa_nz" ∷ ⌜a ≠ 0⌝%N -∗
+      "%Hrepmem" ∷ ⌜N_nat_repr (sr_mem_mm sr) (rt_memaddr sr MemMM)⌝ -∗
+      "%Hmemmm" ∷ ⌜inst_memory (f_inst f) !! base_mem_idx mr MemMM = Some (sr_mem_mm sr)⌝ -∗
+      "%Hmemgc" ∷ ⌜inst_memory (f_inst f) !! base_mem_idx mr MemGC = Some (sr_mem_gc sr)⌝ -∗
+      "HΦ" ∷
+        (∀ f' vs vsf ns',
+           "Hptr"  ∷ ℓ ↦heap update_path_words off ws (map WordInt ns') -∗
+           "Haddr" ∷ ℓ ↦addr (MemMM, a) -∗
+           "Hown"  ∷ na_own logrel_nais E -∗
+           "Htok"  ∷ rt_token rti sr lmask θ -∗
+           "Hregf" ∷ instance_rt_func_interp mr.(mr_func_registerroot) sr.(sr_func_registerroot) (spec_registerroot rti sr) f.(f_inst) -∗
+           "Hos"    ∷ ([∗ list] o;v ∈ os; vs, atom_interp o v) -∗
+           "%Hns'" ∷ ⌜length ns' = areps_size ιs⌝ -∗
+           "%Hf'"  ∷ ⌜f' = mk_load_frame fe f wl vsf⌝ -∗
+           "%Hvsf" ∷ ⌜Forall2 (λ ι vf, types_agree (translate_arep ι) vf) ιs vsf⌝ -∗
+           Φ f' vs) -∗
+      CWP es @ E UNDER B; R {{ Φ }}.
+  Proof.
+    induction ιs as [| ιs ι] using seq.last_ind; intros * Hcg *.
+    - cbn in Hcg.
+      inversion Hcg; subst ret wt' wl' es.
+      repeat (split; first done).
+      intros *.
+      repeat iIntros "@".
+      iApply (cwp_nil with "[$] [$]").
+      inversion Harep; subst.
+      iApply ("HΦ" $! f [] [] [] with "[Hptr] [$Haddr] [$Hown] [$Htok] [$Hregf] [$]"); try done; [].
+      by rewrite update_path_words_empty_2.
+    - apply inv_foldlM_rcons in Hcg.
+      destruct Hcg as (n & ?wt & ?wt & ?wl & ?wl & es_fold & es_load & Hfold & Hload & -> & -> & ->).
+      inv_cg_bind Hload ?ret ?wt ?wt ?wl ?wl es_load1 ?es_rest Hload1 Hret.
+      inv_cg_ret Hret; subst; clear_nils.
+      pose proof (IHιs se _ _ _ _ _ _ _ _ _ Hfold) as (-> & -> & -> & IHspec).
+      pose proof (wp_mem_load1_cg_state rti sr mr _ _ _ _ _ _ _ _ _ _ _ _ Hload1) as (-> & -> & ->).
+      split.
+      { by rewrite seq.foldl_rcons. }
+      split.
+      { done. }
+      split.
+      { by rewrite rcons_app map_app. }
+      intros *.
+      repeat iIntros "@".
+      apply Forall2_rcons_inv_l in Harep.
+      destruct Harep as (o & os' & Ho & Hos & ->).
+      rename os' into os.
+
+      iApply (cwp_seq with "[-HΦ]").
+      {
+        apply Forall2_rcons_inv_l in Hser.
+        destruct Hser as ([off' sz'] & offs_szs' & Hoffsz & Hser' & Hoffs_szs).
+        rename Hser' into Hser.
+        iPoseProof (IHspec with "[$] [$] [$] [$] [//] [$] [$] [$] [//]") as "IH".
+        iApply "IH"; try done.
+        - iPureIntro.
+          rewrite sum_list_with_rcons in Hbound.
+          lia.
+        - iPureIntro.
+          unfold offs_szs, offs in Hoffs_szs.
+          rewrite seq.foldl_rcons in Hoffs_szs.
+          rewrite -> seq.map_rcons in Hoffs_szs.
+          destruct (seq.foldl (λ '(off', offs) (ι : atomic_rep), (off' + arep_size ι, seq.rcons offs off')) (
+                        off, []) ιs) as [off0 offs0] eqn:Heqfold.
+          assert (seq.size offs0 = seq.size (seq.map arep_size ιs)).
+          { admit. }
+          cbn in Hoffs_szs.
+          rewrite seq.zip_rcons in Hoffs_szs; last done.
+          eapply seq.rcons_inj in Hoffs_szs.
+          inversion Hoffs_szs; subst.
+          apply Hser.
+        - rewrite length_app in Hfsz; cbn in Hfsz.
+          iPureIntro.
+          cbn.
+          lia.
+        - iIntros (f' vs' vsf' ns').
+          repeat iIntros "@".
+          instantiate (1 :=
+            (λ f' vs',
+              ∃ vsf' ns',
+                ⌜f' = mk_load_frame (fe_of_context F) f wl vsf'⌝ ∗
+                ([∗ list] o;v ∈ os;vs', atom_interp o v) ∗
+                ⌜Forall2 (λ (ι : atomic_rep) (vf : value), types_agree (translate_arep ι) vf) ιs vsf'⌝ ∗
+                "Hptr" ∷ ℓ ↦heap update_path_words off ws (map WordInt ns') ∗
+                "%Hns'" ∷ ⌜length ns' = areps_size ιs⌝ ∗
+                ?[Q])%I).
+          iExists vsf'.
+          iFrame.
+          iSplitR; first done.
+          iSplitR; first done.
+          iSplitR; first done.
+          iNamedAccu.
+      }
+      iIntros (f' vs') "(%vsf' & %ns' & -> & Hats & %Htys & Hrest) Hf Hr".
+      repeat iDestruct "Hrest" as "[@ Hrest]"; iDestruct "Hrest" as "@".
+      iApply cwp_val_app; first apply has_values_to_consts.
+      iApply (wp_load1_move_mm with "[$] [$] [$] [$] [$] [$] [Hregf] [//] [//] []");
+        first eassumption;
+        try done.
+      + by rewrite load_frame_inst.
+      + admit.
+      + admit.
+      + admit.
+      + iPureIntro.
+        by rewrite mk_load_frame_stable_part.
+      + by rewrite load_frame_inst.
+      + by rewrite load_frame_inst.
+      + iIntros (f' vf' v' ns'').
+        repeat iIntros "@".
+        iApply ("HΦ" with "[Hptr] [Haddr] [$Hown] [$Htok] [Hregf] [Hats Ho] [] [] []").
+        * by erewrite update_update_wordint.
+        * done.
+        * by rewrite load_frame_inst.
+        * rewrite rcons_app.
+          iApply (big_sepL2_app with "[Hats]"); iFrame.
+          done.
+        * iPureIntro.
+          rewrite length_app rcons_app Hns' Hns'0.
+          unfold areps_size, compose.
+          rewrite map_app list_sum_app.
+          cbn.
+          lia.
+        * rewrite length_app length_map in Hf'.
+          pose proof (Forall2_length _ _ _ Htys) as Hvsflen.
+          rewrite Hvsflen in Hf'.
+          rewrite mk_frame_rcons in Hf'; eauto.
+        * iPureIntro.
+          rewrite rcons_app.
+          apply Forall2_app; first done.
+          by constructor.
+  Admitted.
+
+  Lemma wp_mem_load_move (se : @semantic_env Σ) F lidx off ιs wt wl ret wt' wl' es :
+    let fe := fe_of_context F in
+    run_codegen (memory.load mr fe MemMM Move lidx off ιs) wt wl = inr (ret, wt', wl', es) →
+    let offs := snd $ seq.foldl (λ '(off', offs) ι, (off' + arep_size ι, seq.rcons offs off'))
+                  (off, []) ιs in
+    let offs_szs := seq.zip offs (map arep_size ιs) in
+    ret = () /\
+    wt' = [] ∧
+    wl' = map translate_arep ιs ∧
+    ∀ f ℓ a32 a os ws E B R θ lmask Φ,
+    ⊢ "Hf" ∷ ↪[frame] f -∗
+      "Hrun" ∷ ↪[RUN] -∗
+      "Hptr" ∷ ℓ ↦heap ws -∗
+      "Haddr" ∷ ℓ ↦addr (MemMM, a) -∗
+      "%Hℓmask"  ∷ ⌜¬ lmask ℓ⌝ -∗
+      "Hown"  ∷ na_own logrel_nais E -∗
+      "Htok"  ∷ rt_token rti sr lmask θ -∗
+      "Hregf" ∷ instance_rt_func_interp mr.(mr_func_registerroot) sr.(sr_func_registerroot) (spec_registerroot rti sr) f.(f_inst) -∗
+      "%Hmask" ∷ ⌜↑ns_fun (N.of_nat (sr_func_registerroot sr)) ⊆ E⌝ -∗
+      "%Hbound" ∷ ⌜off + sum_list_with arep_size ιs ≤ length ws⌝ -∗
+      "%Harep" ∷ ⌜Forall2 has_arep ιs os⌝ -∗
+      "%Hser" ∷ ⌜Forall2 (λ o '(off, sz), serialize_atom o = get_path_words off sz ws) os offs_szs⌝ -∗
+      "%Hse" ∷ ⌜sem_env_interp F se⌝ -∗
+      "%Hfsz" ∷ ⌜fe_wlocal_offset fe + length wl + length wl' <= length (f_locs f)⌝ -∗
+      "%Hlidx" ∷ ⌜f_locs f !! localimm lidx = Some (VAL_int32 a32)⌝ -∗
+      "%Hlidx_bdd" ∷ ⌜localimm lidx < fe_wlocal_offset fe + length wl⌝ -∗
+      "%Hrepa" ∷ ⌜N_i32_repr (tag_address MemMM a) a32⌝ -∗
+      "%Hrepa_mod" ∷ ⌜a `mod` 4 = 0⌝%N -∗
+      "%Hrepa_nz" ∷ ⌜a ≠ 0⌝%N -∗
+      "%Hrepmem" ∷ ⌜N_nat_repr (sr_mem_mm sr) (rt_memaddr sr MemMM)⌝ -∗
+      "%Hmemmm" ∷ ⌜inst_memory (f_inst f) !! base_mem_idx mr MemMM = Some (sr_mem_mm sr)⌝ -∗
+      "%Hmemgc" ∷ ⌜inst_memory (f_inst f) !! base_mem_idx mr MemGC = Some (sr_mem_gc sr)⌝ -∗
+      "HΦ" ∷
+        (∀ f' vs vsf ns',
+           "%Hns'" ∷ ⌜length ns' = areps_size ιs⌝ -∗
+           "%Hf'"  ∷ ⌜f' = mk_load_frame fe f wl vsf⌝ -∗
+           "%Hvsf" ∷ ⌜Forall2 (λ ι vf, types_agree (translate_arep ι) vf) ιs vsf⌝ -∗
+           "Hptr"  ∷ ℓ ↦heap update_path_words off ws (map WordInt ns') -∗
+           "Haddr" ∷ ℓ ↦addr (MemMM, a) -∗
+           "Hown"  ∷ na_own logrel_nais E -∗
+           "Htok"  ∷ rt_token rti sr lmask θ -∗
+           "Hregf" ∷ instance_rt_func_interp mr.(mr_func_registerroot) sr.(sr_func_registerroot) (spec_registerroot rti sr) f.(f_inst) -∗
+           "Hos"    ∷ ([∗ list] o;v ∈ os; vs, atom_interp o v) -∗
+           Φ f' vs) -∗
+      CWP es @ E UNDER B; R {{ Φ }}.
+  Proof.
+    iIntros (? Hcg ? ?).
+    apply wp_ignore in Hcg.
+    destruct Hcg as (-> & ret' & Hcg).
+    pose proof (wp_mem_load_move_inner _ se _ _ _ _ _ _ _ _ _ Hcg)
+     as (-> & -> & -> & Hspec).
+    split; first done.
+    split; first done.
+    split; first done.
+    intros *.
+    repeat iIntros "@".
+    iPoseProof Hspec as "Hspec".
+    repeat iSpecialize ("Hspec" with "[$]").
+    repeat iSpecialize ("Hspec" with "[//]").
+    repeat iSpecialize ("Hspec" with "[$]").
+    iApply "Hspec"; eauto.
+    iIntros (f' vs' vsf' ns').
+    repeat iIntros "@".
+    iApply ("HΦ" with "[//] [//] [//] [$] [$] [$] [$] [$] [$]").
+  Qed.
+
+End load_move.
