theories/iris/logrel/rt_token.v
@@ -1,0 +1,41 @@
+Require Import RichWasm.iris.memory.
+Require Import RichWasm.iris.logrel.
+Require Import RichWasm.iris.util.
+Require Import RichWasm.util.
+From iris.proofmode Require Import base proofmode classes.
+
+Set Bullet Behavior "Strict Subproofs".
+Set Default Goal Selector "!".
+
+
+Section rt_token.
+  Context `{!logrel_na_invs Σ}.
+  Context `{!wasmG Σ}.
+  Context `{!richwasmG Σ}.
+
+  Variable rti : rt_invariant Σ.
+  Variable sr : store_runtime.
+
+  Lemma rt_token_getheap lmask θ :
+    rt_token rti sr lmask θ -∗
+    ∃ hm,
+      rt_token_phys sr θ hm ∗
+      rt_token_nophys rti sr lmask θ hm.
+  Proof.
+    iIntros "Hrt".
+    open_rt "Hrt".
+    by iFrame.
+  Qed.
+
+  Lemma rt_token_putheap lmask θ hm :
+    rt_token_nophys rti sr lmask θ hm -∗
+    rt_token_phys sr θ hm -∗
+    rt_token rti sr lmask θ.
+  Proof.
+    iIntros "Hnph Hph".
+    iDestruct "Hnph" as "(%rm & %lm & Hnoheap)".
+    iDestruct "Hph" as "(? & ? & ?)".
+    iExists rm, lm, hm.
+    by iFrame.
+  Qed.
+End rt_token.
